updated inv and ind_inv

src/proofs/no_slashable_blocks/supporting_lemmas/ind_inv.dfy
@@ -1,20 +1,25 @@
-include "../../../common/commons.dfy"
-include "../common/attestation_creation_instrumented.dfy"
-include "../../../specs/consensus/consensus.dfy"
-include "../../../specs/network/network.dfy"
-include "../../../specs/dv/dv_attestation_creation.dfy"
+include "../../../common/block_proposer/block_types.dfy"
+include "../../../common/block_proposer/block_common_functions.dfy"
+include "../../../common/block_proposer/block_signing_functions.dfy"
+include "../../../specs/consensus/block_consensus.dfy"
+include "../../../specs/network/block_network.dfy"
+include "../../../specs/dv/dv_block_proposer.dfy"
+include "../common/dvc_block_proposer_instrumented.dfy"
+include "../../common/helper_sets_lemmas.dfy"
+include "../common/block_dvc_spec_axioms.dfy"
 include "inv.dfy"
 
 
-module Att_Ind_Inv_With_Empty_Init_Att_Slashing_DB
+module Block_Ind_Inv_With_Empty_Initial_Block_Slashing_DB
 {
-    import opened Types 
-    import opened CommonFunctions
-    import opened ConsensusSpec
-    import opened NetworkSpec
-    import opened DVC_Spec
-    import opened DV
-    import opened Att_Inv_With_Empty_Initial_Attestation_Slashing_DB
+    import opened Block_Types 
+    import opened Block_Common_Functions
+    import opened Block_Signing_Functions
+    import opened Block_Consensus_Spec
+    import opened Block_Network_Spec
+    import opened DVC_Block_Proposer_Spec_Instr
+    import opened DV_Block_Proposer_Spec
+    import opened Block_Inv_With_Empty_Initial_Block_Slashing_DB
 
     predicate ind_inv(dv: DVState)       
     {
@@ -32,117 +37,134 @@ module Att_Ind_Inv_With_Empty_Init_Att_Slashing_DB
         && invs_group_12(dv)      
         && invs_group_13(dv)  
         && invs_group_14(dv)  
+        && invs_group_15(dv)  
     }
 
     predicate invs_group_1(dv: DVState)       
     {
         &&  inv_quorum_constraints(dv)
         &&  inv_unchanged_paras_of_consensus_instances(dv)
-        &&  inv_only_dv_construct_signed_attestation_signature(dv)
-        &&  inv_current_att_duty_is_rcvd_duty(dv)
+        &&  inv_only_dv_construct_complete_signing_functions(dv)
+        &&  inv_current_proposer_duty_is_rcvd_duty(dv)
         &&  inv_latest_served_duty_is_rcvd_duty(dv)
     }
 
     predicate invs_group_2(dv: DVState)       
     {        
-        &&  inv_none_latest_served_duty_implies_none_current_att_duty(dv)   
-        &&  inv_current_att_duty_is_either_none_or_latest_served_duty(dv)  
-        &&  inv_available_current_att_duty_is_latest_served_att_duty(dv) 
-        &&  inv_is_sequence_attestation_duties_to_be_serves_orders(dv)              
+        &&  inv_none_latest_served_duty_implies_none_current_proposer_duty(dv)   
+        &&  inv_current_proposer_duty_is_either_none_or_latest_served_duty(dv)  
+        &&  inv_available_current_proposer_duty_is_latest_served_proposer_duty(dv) 
     }
 
     predicate invs_group_3(dv: DVState)       
     {        
-        &&  inv_no_duplicated_att_duties(dv)           
-        &&  inv_every_att_duty_before_dvn_att_index_was_delivered(dv) 
-        &&  inv_no_active_consensus_instance_before_receiving_an_att_duty(dv)              
+        &&  inv_no_duplicated_proposer_duties(dv)           
+        &&  inv_every_proposer_duty_before_dvn_proposer_index_was_delivered(dv) 
+        &&  inv_no_active_consensus_instance_before_receiving_a_proposer_duty(dv)              
     }
 
     predicate invs_group_4(dv: DVState)       
     {        
-        &&  inv_slot_of_active_consensus_instance_is_not_higher_than_slot_of_latest_served_att_duty(dv)  
-        &&  inv_consensus_instance_only_for_slot_in_which_dvc_has_rcvd_att_duty(dv)          
+        &&  inv_slot_of_active_consensus_instance_is_not_higher_than_slot_of_latest_served_proposer_duty(dv)  
+        &&  inv_consensus_instance_only_for_slot_in_which_dvc_has_rcvd_proposer_duty(dv)          
         &&  inv_consensus_instances_only_for_rcvd_duties(dv)  
-        &&  inv_rcvd_att_duty_is_from_dv_seq_for_rcvd_att_duty(dv)
+        &&  inv_rcvd_proposer_duty_is_from_dv_seq_for_rcvd_proposer_duty(dv)
     }
 
     predicate invs_group_5(dv: DVState)       
     {                
-        &&  inv_att_slashing_db_hist_keeps_track_of_only_rcvd_att_duties(dv)  
-        &&  inv_exists_db_in_att_slashing_db_hist_and_duty_for_every_validity_predicate(dv)  
-        &&  inv_current_validity_predicate_for_slot_k_is_stored_in_att_slashing_db_hist_k(dv)          
+        &&  inv_block_slashing_db_hist_keeps_track_of_only_rcvd_proposer_duties(dv)  
+        &&  inv_exists_db_in_block_slashing_db_hist_and_proposer_duty_and_randao_reveal_for_every_validity_predicate(dv)  
+        &&  inv_current_validity_predicate_for_slot_k_is_stored_in_block_slashing_db_hist_k(dv)          
     }
 
     predicate invs_group_6(dv: DVState)       
     {                
-        &&  inv_every_db_in_att_slashing_db_hist_is_subset_of_att_slashing_db(dv)  
-        &&  inv_active_attn_consensus_instances_are_tracked_in_att_slashing_db_hist(dv)
-        &&  inv_construct_signed_attestation_signature_assumptions_helper(dv)        
+        &&  inv_every_db_in_block_slashing_db_hist_is_subset_of_block_slashing_db(dv)  
+        &&  inv_active_consensus_instances_on_beacon_blocks_are_tracked_in_block_slashing_db_hist(dv)
+
+        // &&  inv_construct_signed_attestation_signature_assumptions_helper(dv)        
     }
 
     predicate invs_group_7(dv: DVState)       
     {                
         &&  inv_all_in_transit_messages_were_sent(dv)
-        &&  inv_rcvd_attn_shares_are_from_sent_messages(dv)
-        &&  inv_slots_for_sent_validity_predicate_are_stored_in_att_slashing_db_hist(dv)
+        &&  inv_rcvd_block_shares_are_from_sent_messages(dv)
+        &&  inv_slots_for_sent_validity_predicate_are_stored_in_block_slashing_db_hist(dv)
     }
     
     predicate invs_group_8(dv: DVState)       
-    {                
-        && inv_all_validity_predicates_are_stored_in_att_slashing_db_hist(dv)
-        && inv_exists_honest_dvc_that_sent_att_share_for_submitted_att(dv) 
+    {   
+        && inv_exists_honest_dvc_that_sent_block_share_for_submitted_block(dv) 
         && inv_decided_value_of_consensus_instance_is_decided_by_quorum(dv)    
-        && inv_sent_validity_predicate_is_based_on_rcvd_att_duty_and_slashing_db_for_dv(dv)
-        && inv_sent_validity_predicate_is_based_on_rcvd_att_duty_and_slashing_db(dv)
-        
+        && inv_sent_validity_predicate_is_based_on_rcvd_proposer_duty_and_slashing_db_and_randao_reveal_for_dv(dv)
+        && inv_sent_validity_predicate_is_based_on_rcvd_proposer_duty_and_slashing_db_and_randao_reveal(dv)
     }
 
     predicate invs_group_9(dv: DVState)       
     {                    
         && inv_decided_value_of_consensus_instance_of_slot_k_is_for_slot_k(dv) 
         && invNetwork(dv)
-        && inv_attestation_shares_to_broadcast_are_sent_messages(dv)
-        && inv_attestation_shares_to_broadcast_is_a_subset_of_all_messages_sent(dv)
+        && inv_block_shares_to_broadcast_are_sent_messages(dv)
+
+        // Move to intermediate steps
+        && inv_block_shares_to_broadcast_is_a_subset_of_all_sent_messages(dv)
+
+        
     }
 
     predicate invs_group_10(dv: DVState)       
-    {                
-        && inv_exists_att_duty_in_dv_seq_of_att_duty_for_every_slot_in_att_slashing_db_hist(dv)        
-        && inv_available_latest_attestation_duty_is_from_dv_seq_of_att_duties(dv)
-        && inv_exists_att_duty_in_dv_seq_of_att_duty_for_every_slot_in_att_slashing_db_hist_a(dv)        
-        && inv_data_of_att_share_is_decided_value(dv)                     
+    {   
+        && inv_available_latest_proposer_duty_is_from_dv_seq_of_proposer_duties(dv)        
+        && inv_exists_proposer_duty_in_dv_seq_of_proposer_duties_for_every_slot_in_block_slashing_db_hist(dv) 
+        && inv_block_of_in_transit_block_share_is_decided_value(dv)                     
+
+        // Move to intermediate steps
+        && inv_available_current_proposer_duty_is_from_dv_seq_of_proposer_duties(dv)                 
+        
     }
     
     predicate invs_group_11(dv: DVState)       
-    {                
+    {             
+        && inv_slot_in_future_beacon_block_is_correct(dv)  
         && inv_future_decided_data_of_dvc_is_consistent_with_existing_decision_dv(dv)
-        && inv_slot_in_future_decided_data_is_correct(dv)  
+        && inv_none_latest_proposer_duty_and_empty_set_of_rcvd_proposer_duties(dv)
+        && inv_unique_rcvd_proposer_duty_per_slot(dv)
     }
     
     predicate invs_group_12(dv: DVState)       
-    {                
-        && inv_sent_validity_predicate_only_for_slots_stored_in_att_slashing_db_hist(dv)
-        && inv_all_validity_predicates_are_stored_in_att_slashing_db_hist(dv)
-        && inv_consensus_instances_are_isConditionForSafetyTrue(dv)
-        && inv_none_latest_att_duty_and_empty_set_of_rcvd_att_duties(dv)
-        && inv_unique_rcvd_att_duty_per_slot(dv)
-        && inv_no_rcvd_att_duty_is_higher_than_latest_att_duty(dv)
+    {   
+        && inv_consensus_instance_isConditionForSafetyTrue(dv)
+        && inv_no_rcvd_proposer_duty_is_higher_than_latest_proposer_duty(dv)
+        && inv_sent_validity_predicate_only_for_slots_stored_in_block_slashing_db_hist(dv)
+        && inv_all_validity_predicates_are_stored_in_block_slashing_db_hist(dv)
+        
     }
 
     predicate invs_group_13(dv: DVState)       
     {   
-        && inv_decided_data_has_an_honest_witness(dv)
-        && inv_all_created_attestations_are_valid(dv)
-        && inv_attestation_is_created_with_shares_from_quorum(dv)
         && inv_unchanged_dvc_rs_pubkey(dv)
+        && inv_all_created_signed_beacon_blocks_are_valid(dv)
+        && inv_complete_block_is_created_with_shares_from_quorum(dv)
+        && inv_exists_an_honest_dvc_as_a_witness_for_every_decided_beacon_block(dv)
+
+        // Move to intermediate steps
+        // && inv_proposer_duty_in_next_delivery_is_higher_than_latest_served_proposer_duty(dv)
     }
 
     predicate invs_group_14(dv: DVState)       
     {   
-        && inv_sequence_attestation_duties_to_be_served_ordered(dv)
-        && inv_att_shares_to_broadcast_is_tracked_in_attestation_slashing_db(dv)
-        && inv_data_of_att_shares_is_known(dv)
-        && inv_slot_of_consensus_instance_is_up_to_slot_of_latest_attestation_duty(dv)
-        && inv_db_of_vp_contains_all_att_data_of_sent_att_shares_for_lower_slots(dv)
+        && inv_seq_of_proposer_duties_is_ordered(dv)
+        && inv_block_shares_to_broadcast_is_tracked_in_block_slashing_db(dv)
+        && inv_block_of_block_shares_is_known(dv)
+        && inv_slot_of_consensus_instance_is_up_to_slot_of_latest_proposer_duty(dv)
+        && inv_db_of_vp_contains_all_beacon_block_of_sent_block_shares_for_lower_slots(dv)
+    }
+
+    predicate invs_group_15(dv: DVState)       
+    {   
+        && inv_none_latest_proposer_duty_implies_emply_block_slashing_db(dv)
+        && inv_slots_in_slashing_db_is_not_higher_than_slot_of_latest_proposer_duty(dv)
+        && inv_at_most_submitted_signed_beacon_block_for_every_slot(dv)
     }
 }
