src/proofs/no_slashable_blocks/supporting_lemmas/inv.dfy
@@ -50,7 +50,7 @@ module Block_Inv_With_Empty_Initial_Block_Slashing_DB
                && |ci.all_nodes - ci.honest_nodes_status.Keys| <= f(|ci.all_nodes|)
     }
 
-    predicate same_honest_nodes_in_dv_and_ci(dv: DVState)
+    predicate inv_same_node_status_in_dv_and_ci(dv: DVState)
     {
         forall s: Slot ::
             && var ci := dv.consensus_instances_on_beacon_block[s];            
@@ -92,7 +92,7 @@ module Block_Inv_With_Empty_Initial_Block_Slashing_DB
                 && nodes.peers == dv.all_nodes
     }
 
-    predicate inv_only_dv_construct_complete_signature_functions(dv: DVState)
+    predicate inv_only_dv_construct_complete_signing_functions(dv: DVState)
     {
         && inv_only_dv_construct_complete_signed_randao_reveal(dv)
         && inv_only_dv_construct_complete_signed_block(dv)                
@@ -183,7 +183,7 @@ module Block_Inv_With_Empty_Initial_Block_Slashing_DB
                 && duty1.slot < duty2.slot
     }
 
-    predicate inv_unchanged_dvn_seq_of_proposer_duties(dv: DVState, dv': DVState)
+    predicate inv_unchanged_dv_seq_of_proposer_duties(dv: DVState, dv': DVState)
     {
         dv.sequence_proposer_duties_to_be_served
                 == dv'.sequence_proposer_duties_to_be_served
@@ -203,7 +203,38 @@ module Block_Inv_With_Empty_Initial_Block_Slashing_DB
             && inv_no_active_consensus_instance_before_receiving_a_proposer_duty_body(dvc)
     }
 
-    predicate pred_proposer_duty_is_from_dv_seq_of_proposer_duties_new_body(  
+
+    predicate inv_available_current_proposer_duty_is_from_dv_seq_of_proposer_duties_body(  
+        dvc: DVCState,
+        hn: BLSPubkey,
+        sequence_proposer_duties_to_be_served: iseq<ProposerDutyAndNode>,    
+        index_next_proposer_duty_to_be_served: nat
+    )
+    {
+        dvc.current_proposer_duty.isPresent()
+        ==>
+        (   && var proposer_duty := dvc.current_proposer_duty.safe_get();
+            && exists i: Slot :: 
+                    && i < index_next_proposer_duty_to_be_served
+                    && var an := sequence_proposer_duties_to_be_served[i];
+                    && an.proposer_duty == proposer_duty
+                    && an.node == hn
+        )
+    } 
+
+    predicate inv_available_current_proposer_duty_is_from_dv_seq_of_proposer_duties(dv: DVState)
+    {
+        forall hn: BLSPubkey | hn in dv.honest_nodes_states.Keys ::
+            && var dvc := dv.honest_nodes_states[hn];
+            && inv_available_current_proposer_duty_is_from_dv_seq_of_proposer_duties_body(
+                    dvc,
+                    hn,
+                    dv.sequence_proposer_duties_to_be_served,
+                    dv.index_next_proposer_duty_to_be_served
+                )
+    }  
+
+    predicate pred_proposer_duty_is_from_dv_seq_of_proposer_duties_body(  
         proposer_duty: ProposerDuty,
         hn: BLSPubkey,
         sequence_proposer_duties_to_be_served: iseq<ProposerDutyAndNode>,    
@@ -217,7 +248,7 @@ module Block_Inv_With_Empty_Initial_Block_Slashing_DB
             && an.node == hn
     }     
 
-    predicate inv_latest_proposer_duty_is_from_dv_seq_of_proposer_duties_helper(  
+    predicate inv_available_latest_proposer_duty_is_from_dv_seq_of_proposer_duties_helper(  
         n: BLSPubkey,
         n_state: DVCState,
         sequence_proposer_duties_to_be_served: iseq<ProposerDutyAndNode>,    
@@ -233,12 +264,12 @@ module Block_Inv_With_Empty_Initial_Block_Slashing_DB
             && an.node == n
     }  
 
-    predicate inv_latest_proposer_duty_is_from_dv_seq_of_proposer_duties(dv: DVState)    
+    predicate inv_available_latest_proposer_duty_is_from_dv_seq_of_proposer_duties(dv: DVState)    
     {
         forall hn |
             && hn in dv.honest_nodes_states.Keys          
             ::
-            inv_latest_proposer_duty_is_from_dv_seq_of_proposer_duties_body(
+            inv_available_latest_proposer_duty_is_from_dv_seq_of_proposer_duties_body(
                 dv, 
                 hn,
                 dv.honest_nodes_states[hn],
@@ -246,7 +277,7 @@ module Block_Inv_With_Empty_Initial_Block_Slashing_DB
             )                    
     }               
 
-    predicate inv_latest_proposer_duty_is_from_dv_seq_of_proposer_duties_body(
+    predicate inv_available_latest_proposer_duty_is_from_dv_seq_of_proposer_duties_body(
         dv: DVState, 
         n: BLSPubkey,
         n_state: DVCState,
@@ -333,6 +364,15 @@ module Block_Inv_With_Empty_Initial_Block_Slashing_DB
          forall m | m in dv.block_share_network.messagesInTransit::
                 m.message in dv.block_share_network.allMessagesSent       
     } 
+    
+    predicate invNetwork(
+        dv: DVState
+    )
+    {
+        forall m | m in dv.block_share_network.messagesInTransit
+            ::
+            m.message in dv.block_share_network.allMessagesSent       
+    }
 
     predicate inv_rcvd_block_shares_are_in_all_sent_messages_body(
         dv: DVState,
@@ -347,15 +387,6 @@ module Block_Inv_With_Empty_Initial_Block_Slashing_DB
             ::
             rcvd_block_shares[i][j] <= dv.block_share_network.allMessagesSent
     }
-    
-    predicate invNetwork(
-        dv: DVState
-    )
-    {
-        forall m | m in dv.block_share_network.messagesInTransit
-            ::
-            m.message in dv.block_share_network.allMessagesSent       
-    }
 
     predicate inv_rcvd_block_shares_are_in_all_sent_messages(
         dv: DVState
@@ -366,6 +397,28 @@ module Block_Inv_With_Empty_Initial_Block_Slashing_DB
             && inv_rcvd_block_shares_are_in_all_sent_messages_body(dv, dvc)
         
     }
+
+    // predicate inv_rcvd_block_shares_are_in_all_messages_dvc(
+    //     dv: DVState,
+    //     n: BLSPubkey
+    // )
+    // requires n in dv.honest_nodes_states.Keys
+    // {
+    //     inv_rcvd_block_shares_are_in_all_sent_messages_body(
+    //         dv,
+    //         dv.honest_nodes_states[n]
+    //     )
+    // }
+
+    // predicate inv_rcvd_block_shares_are_in_all_sent_messages(
+    //     dv: DVState    
+    // )
+    // {
+    //     forall n |
+    //         n in dv.honest_nodes_states
+    //         ::
+    //         inv_rcvd_block_shares_are_in_all_messages_dvc(dv, n)
+    // }  
 
     predicate inv_exists_honest_dvc_that_sent_block_share_for_submitted_block_body(
         dv: DVState,
@@ -391,37 +444,6 @@ module Block_Inv_With_Empty_Initial_Block_Slashing_DB
                 inv_exists_honest_dvc_that_sent_block_share_for_submitted_block_body(dv, hn, block_share, block)
     }
    
-
-
-
-
-    predicate inv_sent_validity_predicate_is_based_on_rcvd_proposer_duty_and_slashing_db_and_randao_reveal_for_dvc_body(
-        dvc: DVCState,
-        cid: Slot
-    )
-    requires cid in dvc.block_consensus_engine_state.active_consensus_instances_on_beacon_blocks
-    {
-        var bci := dvc.block_consensus_engine_state.active_consensus_instances_on_beacon_blocks[cid];
-        inv_existing_block_slashing_db_and_randao_reveal_for_sent_vp(
-            cid, 
-            bci.proposer_duty, 
-            bci.randao_reveal,
-            bci.validityPredicate            
-        ) 
-    }     
-
-   
-
-    predicate inv_sent_validity_predicate_is_based_on_rcvd_proposer_duty_and_slashing_db_and_randao_reveal_for_dvc(
-        dvc: DVCState
-    )
-    {
-        forall cid | 
-            cid in dvc.block_consensus_engine_state.active_consensus_instances_on_beacon_blocks
-            ::
-            inv_sent_validity_predicate_is_based_on_rcvd_proposer_duty_and_slashing_db_and_randao_reveal_for_dvc_body(dvc, cid)        
-    }    
-
     predicate inv_sent_validity_predicate_is_based_on_rcvd_proposer_duty_and_slashing_db_and_randao_reveal_body(
         s: Slot,
         proposer_duty: ProposerDuty,        
@@ -442,14 +464,14 @@ module Block_Inv_With_Empty_Initial_Block_Slashing_DB
             )
     }
 
-    predicate inv_existing_block_slashing_db_and_randao_reveal_for_sent_vp(
+    predicate inv_existing_block_slashing_db_for_sent_vp(
         cid: Slot,
         proposer_duty: ProposerDuty,
         randao_reveal: BLSSignature,
         vp: BeaconBlock -> bool        
     )
     {
-        exists  block_slashing_db: set<SlashingDBBlock>, randao_reveal: BLSSignature
+        exists  block_slashing_db: set<SlashingDBBlock>
                 ::
                 inv_sent_validity_predicate_is_based_on_rcvd_proposer_duty_and_slashing_db_and_randao_reveal_body(
                     cid, 
@@ -458,7 +480,36 @@ module Block_Inv_With_Empty_Initial_Block_Slashing_DB
                     randao_reveal,
                     vp
                 )
-    }      
+    }  
+
+    predicate inv_sent_validity_predicate_is_based_on_rcvd_proposer_duty_and_slashing_db_and_randao_reveal_for_dvc_body(
+        dvc: DVCState,
+        cid: Slot
+    )
+    requires cid in dvc.block_consensus_engine_state.active_consensus_instances_on_beacon_blocks
+    {
+        var bci := dvc.block_consensus_engine_state.active_consensus_instances_on_beacon_blocks[cid];
+        inv_existing_block_slashing_db_for_sent_vp(
+            cid, 
+            bci.proposer_duty, 
+            bci.randao_reveal,
+            bci.validityPredicate            
+        ) 
+    }     
+
+    predicate inv_sent_validity_predicate_is_based_on_rcvd_proposer_duty_and_slashing_db_and_randao_reveal_for_dvc(
+        dvc: DVCState
+    )
+    {
+        forall cid | 
+            cid in dvc.block_consensus_engine_state.active_consensus_instances_on_beacon_blocks
+            ::
+            inv_sent_validity_predicate_is_based_on_rcvd_proposer_duty_and_slashing_db_and_randao_reveal_for_dvc_body(dvc, cid)        
+    }    
+
+
+
+        
 
     predicate inv_sent_validity_predicate_is_based_on_rcvd_proposer_duty_and_slashing_db_and_randao_reveal_for_dvc_single_dvc(
         dv: DVState,
@@ -470,7 +521,7 @@ module Block_Inv_With_Empty_Initial_Block_Slashing_DB
     {
         && var dvc := dv.honest_nodes_states[n];
         && var bci := dvc.block_consensus_engine_state.active_consensus_instances_on_beacon_blocks[cid];
-        && inv_existing_block_slashing_db_and_randao_reveal_for_sent_vp(
+        && inv_existing_block_slashing_db_for_sent_vp(
                 cid, 
                 bci.proposer_duty, 
                 bci.randao_reveal,
@@ -524,7 +575,7 @@ module Block_Inv_With_Empty_Initial_Block_Slashing_DB
             dv.consensus_instances_on_beacon_block[cid].decided_value.safe_get().slot == cid
     }   
 
-    predicate inv_block_of_block_share_is_decided_value(dv: DVState)
+    predicate inv_block_of_in_transit_block_share_is_decided_value(dv: DVState)
     {
         forall hn, block_share |
                 && hn in dv.honest_nodes_states.Keys 
@@ -532,174 +583,313 @@ module Block_Inv_With_Empty_Initial_Block_Slashing_DB
                 && var block_signing_root := compute_block_signing_root(block_share.block);                                      
                 && verify_bls_signature(block_signing_root, block_share.signature, hn)
                 ::
-                inv_block_of_block_share_is_decided_value_body(dv, block_share)
+                inv_block_of_in_transit_block_share_is_decided_value_body(dv, block_share)
     }  
 
-    predicate inv_block_of_block_share_is_decided_value_body(dv: DVState, block_share: SignedBeaconBlock)
+    predicate inv_block_of_in_transit_block_share_is_decided_value_body(dv: DVState, block_share: SignedBeaconBlock)
     {
         && dv.consensus_instances_on_beacon_block[block_share.block.slot].decided_value.isPresent()
         && dv.consensus_instances_on_beacon_block[block_share.block.slot].decided_value.safe_get() == block_share.block
     }  
 
-    // predicate inv_proposer_duty_in_next_delivery_is_not_lower_than_rcvd_proposer_duties_body(dvc: DVCState, next_duty: ProposerDuty)
-    // {
-    //    forall rcvd_duty: ProposerDuty | rcvd_duty in dvc.all_rcvd_duties ::
-    //         rcvd_duty.slot <= next_duty.slot        
-    // }
+    predicate inv_block_shares_to_broadcast_is_a_subset_of_all_sent_messages_body(
+        dv: DVState,
+        n: BLSPubkey
+    )
+    requires n in dv.honest_nodes_states.Keys 
+    {
+        dv.honest_nodes_states[n].block_shares_to_broadcast.Values <= dv.block_share_network.allMessagesSent
+    }
 
-    // predicate inv_proposer_duty_in_next_delivery_is_not_lower_than_rcvd_proposer_duties(dv: DVState)
-    // {
-    //     && var dv_duty_queue := dv.sequence_proposer_duties_to_be_served;
-    //     && var dv_index := dv.index_next_proposer_duty_to_be_served;
-    //     && var next_duty_and_node := dv_duty_queue[dv_index];
-    //     && forall hn: BLSPubkey | 
-    //         && hn in dv.honest_nodes_states.Keys
-    //         && hn == next_duty_and_node.node 
-    //         ::            
-    //         && var dvc := dv.honest_nodes_states[hn];
-    //         && var next_duty := next_duty_and_node.proposer_duty;
-    //         && inv_proposer_duty_in_next_delivery_is_not_lower_than_rcvd_proposer_duties_body(dvc, next_duty)
-    // }
-                  
+    predicate inv_block_shares_to_broadcast_is_a_subset_of_all_sent_messages(
+        dv: DVState
+    )
+    {
+        forall n |
+            n in dv.honest_nodes_states.Keys 
+            ::
+        inv_block_shares_to_broadcast_is_a_subset_of_all_sent_messages_body(dv, n)
+    }  
 
+    predicate inv_block_slashing_db_hist_keeps_track_of_only_rcvd_proposer_duties_body(hn_state: DVCState)    
+    {
+        forall k: Slot | k in hn_state.block_consensus_engine_state.block_slashing_db_hist.Keys ::
+            exists duty: ProposerDuty :: 
+                    && duty in hn_state.all_rcvd_duties
+                    && duty.slot == k
+    }
 
-    // predicate inv_slot_of_active_consensus_instance_is_not_higher_than_slot_of_latest_served_proposer_duty_body(dvc: DVCState)
-    // {
-    //     dvc.latest_proposer_duty.isPresent()
-    //     ==> ( forall k: Slot | k in dvc.block_consensus_engine_state.active_consensus_instances_on_beacon_blocks.Keys 
-    //             ::
-    //             k <= dvc.latest_proposer_duty.safe_get().slot
-    //         )
-    // }
-
-    // predicate inv_slot_of_active_consensus_instance_is_not_higher_than_slot_of_latest_served_proposer_duty(dv: DVState)
-    // {
-    //     forall hn: BLSPubkey | hn in dv.honest_nodes_states.Keys ::
-    //         && var dvc := dv.honest_nodes_states[hn];
-    //         && inv_slot_of_active_consensus_instance_is_not_higher_than_slot_of_latest_served_proposer_duty_body(dvc)
-    // }
+    predicate inv_block_slashing_db_hist_keeps_track_of_only_rcvd_proposer_duties(dv: DVState)
+    {
+        forall hn: BLSPubkey | is_honest_node(dv, hn) ::
+            && var hn_state := dv.honest_nodes_states[hn];            
+            && inv_block_slashing_db_hist_keeps_track_of_only_rcvd_proposer_duties_body(hn_state)       
+    }
 
 
+    predicate inv_exists_db_in_block_slashing_db_hist_and_proposer_duty_and_randao_reveal_for_every_validity_predicate_body_ces(ces: BlockConsensusEngineState)
+    {
+        forall s: Slot, vp: BeaconBlock -> bool |
+                ( && s in ces.block_slashing_db_hist.Keys
+                  && vp in ces.block_slashing_db_hist[s]
+                )
+                :: 
+                ( exists db: set<SlashingDBBlock>, duty: ProposerDuty, randao_reveal: BLSSignature ::
+                        && duty.slot == s
+                        && db in ces.block_slashing_db_hist[s][vp]
+                        && vp == (block: BeaconBlock) => ci_decision_is_valid_beacon_block(db, block, duty, randao_reveal)
+                )
+    }
 
-    // predicate inv_rcvd_block_shares_are_in_all_messages_sent_single_node(
-    //     dv: DVState,
-    //     n: BLSPubkey
-    // )
-    // requires n in dv.honest_nodes_states.Keys
-    // {
-    //     inv_rcvd_block_shares_are_in_all_sent_messages_body(
-    //         dv,
-    //         dv.honest_nodes_states[n]
-    //     )
-    // }
+    predicate inv_exists_db_in_block_slashing_db_hist_and_proposer_duty_and_randao_reveal_for_every_validity_predicate_body(hn_state: DVCState)
+    {
+        forall s: Slot, vp: BeaconBlock -> bool |
+                ( && s in hn_state.block_consensus_engine_state.block_slashing_db_hist.Keys
+                  && vp in hn_state.block_consensus_engine_state.block_slashing_db_hist[s]
+                )
+                :: 
+                ( exists db: set<SlashingDBBlock>, duty: ProposerDuty, randao_reveal: BLSSignature ::
+                        && duty.slot == s
+                        && db in hn_state.block_consensus_engine_state.block_slashing_db_hist[s][vp]
+                        && vp == (block: BeaconBlock) => ci_decision_is_valid_beacon_block(db, block, duty, randao_reveal)
+                )
+    }
 
-    // predicate inv_rcvd_block_shares_are_in_all_messages_sent(
-    //     dv: DVState    
-    // )
-    // {
-    //     forall n |
-    //         n in dv.honest_nodes_states
-    //         ::
-    //         inv_rcvd_block_shares_are_in_all_messages_sent_single_node(dv, n)
-    // }  
+    predicate inv_exists_db_in_block_slashing_db_hist_and_proposer_duty_and_randao_reveal_for_every_validity_predicate(dv: DVState)
+    {
+        forall hn: BLSPubkey | is_honest_node(dv, hn) ::
+            && var dvc := dv.honest_nodes_states[hn];
+            && inv_exists_db_in_block_slashing_db_hist_and_proposer_duty_and_randao_reveal_for_every_validity_predicate_body(dvc)
+    }
 
-    
+    predicate inv_current_validity_predicate_for_slot_k_is_stored_in_block_slashing_db_hist_k_body(hn_state: DVCState)
+    {
+        forall k: Slot |
+            k in hn_state.block_consensus_engine_state.active_consensus_instances_on_beacon_blocks.Keys ::
+                && var ci := hn_state.block_consensus_engine_state.active_consensus_instances_on_beacon_blocks[k];
+                && var vp: BeaconBlock -> bool := ci.validityPredicate;
+                && k in hn_state.block_consensus_engine_state.block_slashing_db_hist.Keys 
+                && vp in hn_state.block_consensus_engine_state.block_slashing_db_hist[k].Keys             
+    }
+
+    predicate inv_current_validity_predicate_for_slot_k_is_stored_in_block_slashing_db_hist_k(dv: DVState)
+    {
+        forall hn: BLSPubkey | is_honest_node(dv, hn) ::
+            && var dvc := dv.honest_nodes_states[hn];
+            && inv_current_validity_predicate_for_slot_k_is_stored_in_block_slashing_db_hist_k_body(dvc)
+    }    
+
+    predicate inv_block_slashing_db_hist_is_monotonic_dvc(dvc: DVCState, dvc': DVCState)
+    {        
+        dvc.block_consensus_engine_state.block_slashing_db_hist.Keys
+        <= 
+        dvc'.block_consensus_engine_state.block_slashing_db_hist.Keys
+    }
+
+    predicate inv_monotonic_block_slashing_db_hist(dv: DVState, event: DV_Block_Proposer_Spec.Event, dv': DVState)    
+    {
+        forall hn: BLSPubkey | is_honest_node(dv, hn) ::
+            && hn in dv'.honest_nodes_states
+            && var dvc := dv.honest_nodes_states[hn];
+            && var dvc' := dv'.honest_nodes_states[hn];
+            && inv_block_slashing_db_hist_is_monotonic_dvc(dvc, dvc')
+    }
+
+    predicate inv_monotonic_set_of_created_blocks(dv: DVState, event: DV_Block_Proposer_Spec.Event, dv': DVState)    
+    {
+        dv.all_blocks_created <= dv'.all_blocks_created
+    }
+
+    predicate inv_every_db_in_block_slashing_db_hist_is_subset_of_block_slashing_db_body_ces(ces: BlockConsensusEngineState, block_slashing_db: set<SlashingDBBlock>)
+    {
+        forall s: Slot, vp: BeaconBlock -> bool, db: set<SlashingDBBlock> |
+                ( && s in ces.block_slashing_db_hist.Keys
+                  && vp in ces.block_slashing_db_hist[s]
+                  && db in ces.block_slashing_db_hist[s][vp]
+                )
+                :: 
+                db <= block_slashing_db
+    }
+
+    predicate inv_every_db_in_block_slashing_db_hist_is_subset_of_block_slashing_db_body(hn_state: DVCState)
+    {
+        forall s: Slot, vp: BeaconBlock -> bool, db: set<SlashingDBBlock> |
+                ( && s in hn_state.block_consensus_engine_state.block_slashing_db_hist.Keys
+                  && vp in hn_state.block_consensus_engine_state.block_slashing_db_hist[s].Keys
+                  && db in hn_state.block_consensus_engine_state.block_slashing_db_hist[s][vp]
+                )
+                :: 
+                db <= hn_state.block_slashing_db
+    }
+
+    predicate inv_every_db_in_block_slashing_db_hist_is_subset_of_block_slashing_db(dv: DVState)
+    {
+        forall hn: BLSPubkey | is_honest_node(dv, hn) ::
+            && var dvc := dv.honest_nodes_states[hn];
+            && inv_every_db_in_block_slashing_db_hist_is_subset_of_block_slashing_db_body(dvc)
+    }
 
 
+    predicate inv_block_shares_to_broadcast_are_sent_messages_body(
+        dv: DVState,
+        dvc: DVCState
+    )    
+    {
+        dvc.block_shares_to_broadcast.Values <= dv.block_share_network.allMessagesSent
+    }
 
+    predicate inv_block_shares_to_broadcast_are_sent_messages(
+        dv: DVState
+    )
+    {
+        forall n | n in dv.honest_nodes_states.Keys ::
+            && var dvc := dv.honest_nodes_states[n];
+            && inv_block_shares_to_broadcast_are_sent_messages_body(dv, dvc)
+    }
 
+    predicate inv_rcvd_block_shares_are_from_sent_messages_body(
+        dv: DVState,
+        dvc: DVCState
+    )
+    {
+        var rcvd_block_shares := dvc.rcvd_block_shares;
 
+        forall i, j |
+            && i in rcvd_block_shares.Keys 
+            && j in rcvd_block_shares[i]
+            ::
+            rcvd_block_shares[i][j] <= dv.block_share_network.allMessagesSent
+    }    
+
+    predicate inv_rcvd_block_shares_are_from_sent_messages(
+        dv: DVState    
+    )
+    {
+        forall n | n in dv.honest_nodes_states ::
+            && var dvc := dv.honest_nodes_states[n];
+            && inv_rcvd_block_shares_are_from_sent_messages_body(dv, dvc)
+    } 
+
+    predicate inv_proposer_duty_in_next_delivery_is_not_lower_than_rcvd_proposer_duties_body(dvc: DVCState, next_duty: ProposerDuty)
+    {
+       forall rcvd_duty: ProposerDuty | rcvd_duty in dvc.all_rcvd_duties ::
+            rcvd_duty.slot <= next_duty.slot        
+    }
+
+    predicate inv_proposer_duty_in_next_delivery_is_not_lower_than_rcvd_proposer_duties(dv: DVState)
+    {
+        && var dv_duty_queue := dv.sequence_proposer_duties_to_be_served;
+        && var dv_index := dv.index_next_proposer_duty_to_be_served;
+        && var next_duty_and_node := dv_duty_queue[dv_index];
+        && forall hn: BLSPubkey | 
+            && hn in dv.honest_nodes_states.Keys
+            && hn == next_duty_and_node.node 
+            ::            
+            && var dvc := dv.honest_nodes_states[hn];
+            && var next_duty := next_duty_and_node.proposer_duty;
+            && inv_proposer_duty_in_next_delivery_is_not_lower_than_rcvd_proposer_duties_body(dvc, next_duty)
+    }
+
+    predicate inv_slot_of_active_consensus_instance_is_lower_than_slot_of_latest_served_proposer_duty_body(dvc: DVCState)
+    {
+        dvc.latest_proposer_duty.isPresent()
+        ==> 
+        (   forall k: Slot | k in dvc.block_consensus_engine_state.active_consensus_instances_on_beacon_blocks.Keys 
+            ::
+            k < dvc.latest_proposer_duty.safe_get().slot
+        )
+    }
+
+    predicate inv_slot_of_active_consensus_instance_is_not_higher_than_slot_of_latest_served_proposer_duty_body(dvc: DVCState)
+    {
+        dvc.latest_proposer_duty.isPresent()
+        ==> 
+        (   forall k: Slot | k in dvc.block_consensus_engine_state.active_consensus_instances_on_beacon_blocks.Keys 
+            ::
+            k <= dvc.latest_proposer_duty.safe_get().slot
+        )
+    }
+
+    predicate inv_slot_of_active_consensus_instance_is_not_higher_than_slot_of_latest_served_proposer_duty(dv: DVState)
+    {
+        forall hn: BLSPubkey | hn in dv.honest_nodes_states.Keys ::
+            && var dvc := dv.honest_nodes_states[hn];
+            && inv_slot_of_active_consensus_instance_is_not_higher_than_slot_of_latest_served_proposer_duty_body(dvc)
+    }
+
+    predicate inv_exists_proposer_duty_in_dv_seq_of_proposer_duties_for_every_slot_in_block_slashing_db_hist_body(
+        sequence_proposer_duties_to_be_served: iseq<ProposerDutyAndNode>,
+        n: BLSPubkey,
+        n_state: DVCState,
+        index_next_proposer_duty_to_be_served: nat
+    )
+    {
+        forall slot  |
+            && slot in n_state.block_consensus_engine_state.block_slashing_db_hist
+            ::
+            exists i: Slot :: 
+                && i < index_next_proposer_duty_to_be_served
+                && var pn := sequence_proposer_duties_to_be_served[i];
+                && pn.proposer_duty.slot == slot 
+                && pn.node == n
+    }          
+
+    predicate inv_exists_proposer_duty_in_dv_seq_of_proposer_duties_for_every_slot_in_block_slashing_db_hist(dv: DVState)    
+    {
+        forall hn |
+            && hn in dv.honest_nodes_states.Keys          
+            ::
+            inv_exists_proposer_duty_in_dv_seq_of_proposer_duties_for_every_slot_in_block_slashing_db_hist_body(
+                dv.sequence_proposer_duties_to_be_served, 
+                hn,
+                dv.honest_nodes_states[hn],
+                dv.index_next_proposer_duty_to_be_served
+            )                    
+    }       
+
+    function get_upperlimit_active_instances(
+        n_state: DVCState
+    ): nat 
+    {
+        if n_state.latest_proposer_duty.isPresent() then
+            n_state.latest_proposer_duty.safe_get().slot + 1
+        else
+            0
+    }                
 
   
 
-    
-
-
- 
-
-       
-
-    // predicate inv_exists_proposer_duty_in_dv_seq_of_proposer_duty_for_every_slot_in_block_slashing_db_hist(dv: DVState)    
+    // predicate inv_exists_proposer_duty_in_dv_seq_of_proposer_duties_for_every_slot_in_block_slashing_db_hist(dv: DVState)    
     // {
     //     forall hn |
     //         && hn in dv.honest_nodes_states.Keys          
     //         ::
-    //         inv_exists_proposer_duty_in_dv_seq_of_proposer_duty_for_every_slot_in_block_slashing_db_hist_body(
-    //             dv, 
-    //             hn,
-    //             dv.honest_nodes_states[hn],
-    //             dv.index_next_proposer_duty_to_be_served
-    //         )                    
-    // }       
-
-    // predicate inv_exists_proposer_duty_in_dv_seq_of_proposer_duty_for_every_slot_in_block_slashing_db_hist_body(
-    //     dv: DVState, 
-    //     n: BLSPubkey,
-    //     n_state: DVCState,
-    //     index_next_proposer_duty_to_be_served: nat
-    // )
-    // {
-    //     forall slot  |
-    //         && slot in n_state.block_consensus_engine_state.block_slashing_db_hist
-    //         ::
-    //         exists i: Slot :: 
-    //             && i < index_next_proposer_duty_to_be_served
-    //             && var an := dv.sequence_proposer_duties_to_be_served[i];
-    //             && an.proposer_duty.slot == slot 
-    //             && an.node == n
-    // }   
-
-    // predicate inv_exists_proposer_duty_in_dv_seq_of_proposer_duty_for_every_slot_in_block_slashing_db_hist_a(dv: DVState)    
-    // {
-    //     forall hn |
-    //         && hn in dv.honest_nodes_states.Keys          
-    //         ::
-    //         inv_slot_of_consensus_instance_is_up_to_slot_of_latest_served_proposer_duty(
+    //         inv_slot_of_consensus_instance_is_up_to_slot_of_latest_proposer_duty(
     //             dv, 
     //             hn,
     //             dv.honest_nodes_states[hn]
     //         )                    
-    // }   
+    // }  
 
-    // function get_upperlimit_active_instances(
-    //     n_state: DVCState
-    // ): nat 
-    // {
-    //     if n_state.latest_proposer_duty.isPresent() then
-    //         n_state.latest_proposer_duty.safe_get().slot + 1
-    //     else
-    //         0
-    // }                
+   
+              
+    predicate inv_slot_of_consensus_instance_is_up_to_slot_of_latest_proposer_duty_body(
+        dvc: DVCState       
+    )
+    {
+        forall slot: Slot |
+            && slot in dvc.block_consensus_engine_state.block_slashing_db_hist.Keys
+            ::
+            slot < get_upperlimit_active_instances(dvc)
+    }     
 
-    // predicate inv_slot_of_consensus_instance_is_up_to_slot_of_latest_served_proposer_duty(
-    //     dv: DVState, 
-    //     n: BLSPubkey,
-    //     n_state: DVCState
-    // )
-    // {
-    //     forall slot  |
-    //         && slot in n_state.block_consensus_engine_state.block_slashing_db_hist
-    //         ::
-    //         slot < get_upperlimit_active_instances(n_state)
-    // }      
-
-    // predicate inv_slot_of_consensus_instance_is_up_to_slot_of_latest_proposer_duty_body(
-    //     dvc: DVCState       
-    // )
-    // {
-    //     forall slot: Slot |
-    //         && slot in dvc.block_consensus_engine_state.block_slashing_db_hist
-    //         ::
-    //         slot < get_upperlimit_active_instances(dvc)
-    // }     
-
-    // predicate inv_slot_of_consensus_instance_is_up_to_slot_of_latest_proposer_duty(
-    //     dv: DVState        
-    // )
-    // {
-    //     forall hn: BLSPubkey | is_honest_node(dv, hn) ::
-    //             inv_slot_of_consensus_instance_is_up_to_slot_of_latest_proposer_duty_body(dv.honest_nodes_states[hn])        
-    // }     
+    predicate inv_slot_of_consensus_instance_is_up_to_slot_of_latest_proposer_duty(
+        dv: DVState        
+    )
+    {
+        forall hn: BLSPubkey | is_honest_node(dv, hn) ::
+                inv_slot_of_consensus_instance_is_up_to_slot_of_latest_proposer_duty_body(dv.honest_nodes_states[hn])        
+    }     
     
         
 
@@ -720,117 +910,79 @@ module Block_Inv_With_Empty_Initial_Block_Slashing_DB
     //         0
     // }
 
-    // predicate inv_future_decided_data_of_dvc_is_consistent_with_existing_decision_dv(dv: DVState)    
-    // {
-    //     forall hn |
-    //         && hn in dv.honest_nodes_states.Keys          
-    //         ::
-    //         inv_future_decided_data_of_dvc_is_consistent_with_existing_decision_dv_body(
-    //             dv, 
-    //             hn,
-    //             dv.honest_nodes_states[hn]
-    //         )                    
-    // }       
+    predicate inv_future_decided_data_of_dvc_is_consistent_with_existing_decision_dv_body(
+        dv: DVState, 
+        n: BLSPubkey,
+        n_state: DVCState
+    )
+    {
+        forall slot |
+            && slot in n_state.future_consensus_instances_on_blocks_already_decided.Keys    
+            ::
+            && dv.consensus_instances_on_beacon_block[slot].decided_value.isPresent()
+            && n_state.future_consensus_instances_on_blocks_already_decided[slot] == dv.consensus_instances_on_beacon_block[slot].decided_value.safe_get()
+    }  
 
-    // predicate inv_future_decided_data_of_dvc_is_consistent_with_existing_decision_dv_body(
-    //     dv: DVState, 
-    //     n: BLSPubkey,
-    //     n_state: DVCState
-    // )
-    // {
-    //     forall slot |
-    //         && slot in n_state.future_proposer_consensus_instances_already_decided.Keys
-    //         ::
-    //         && dv.consensus_instances_on_beacon_block[slot].decided_value.isPresent()
-    //         && n_state.future_proposer_consensus_instances_already_decided[slot] == dv.consensus_instances_on_beacon_block[slot].decided_value.safe_get()
-    // }  
+    predicate inv_future_decided_data_of_dvc_is_consistent_with_existing_decision_dv(dv: DVState)    
+    {
+        forall hn |
+            && hn in dv.honest_nodes_states.Keys          
+            ::
+            inv_future_decided_data_of_dvc_is_consistent_with_existing_decision_dv_body(
+                dv, 
+                hn,
+                dv.honest_nodes_states[hn]
+            )                    
+    }       
 
-    // predicate inv_slot_in_future_decided_data_is_correct(dv: DVState)    
-    // {
-    //     forall hn |
-    //         && hn in dv.honest_nodes_states.Keys          
-    //         ::
-    //         inv_slot_in_future_decided_data_is_correct_body(
-    //             dv, 
-    //             hn,
-    //             dv.honest_nodes_states[hn]
-    //         )                    
-    // }              
+    predicate inv_slot_in_future_beacon_block_is_correct_body(
+        n_state: DVCState
+    )
+    {
+        forall slot |
+            && slot in n_state.future_consensus_instances_on_blocks_already_decided.Keys
+            ::
+            n_state.future_consensus_instances_on_blocks_already_decided[slot].slot == slot
+    }  
 
-    // predicate inv_slot_in_future_decided_data_is_correct_body(
-    //     dv: DVState, 
-    //     n: BLSPubkey,
-    //     n_state: DVCState
-    // )
-    // {
-    //     forall slot |
-    //         && slot in n_state.future_proposer_consensus_instances_already_decided
-    //         ::
-    //         n_state.future_proposer_consensus_instances_already_decided[slot].slot == slot
-    // }       
+    predicate inv_slot_in_future_beacon_block_is_correct(dv: DVState)    
+    {
+        forall hn |
+            && hn in dv.honest_nodes_states.Keys          
+            ::
+            inv_slot_in_future_beacon_block_is_correct_body(
+                dv.honest_nodes_states[hn]
+            )                    
+    }              
 
-    // predicate inv_active_consensus_instances_on_beacon_blocks_keys_is_subset_of_block_slashing_db_hist(dv: DVState)    
-    // {
-    //     forall hn |
-    //         && hn in dv.honest_nodes_states.Keys          
-    //         ::
-    //         inv_active_consensus_instances_on_beacon_blocks_keys_is_subset_of_block_slashing_db_hist_body_body(
-    //             dv.honest_nodes_states[hn]
-    //         )                    
-    // }       
+         
 
-    // predicate inv_active_consensus_instances_on_beacon_blocks_keys_is_subset_of_block_slashing_db_hist_body_body
-    // (
-    //     n_state: DVCState
-    // )
-    // {
-    //     n_state.block_consensus_engine_state.active_consensus_instances_on_beacon_blocks.Keys <= n_state.block_consensus_engine_state.block_slashing_db_hist.Keys
-    // }
+    
 
-    // predicate inv_active_consensus_instances_on_beacon_blocks_predicate_is_in_block_slashing_db_hist(dv: DVState)    
-    // {
-    //     forall hn, cid |
-    //         && hn in dv.honest_nodes_states.Keys        
-    //         ::
-    //         inv_active_consensus_instances_on_beacon_blocks_predicate_is_in_block_slashing_db_hist_body(dv.honest_nodes_states[hn], cid)
-             
-    // }       
 
-    // predicate inv_active_consensus_instances_on_beacon_blocks_predicate_is_in_block_slashing_db_hist_body
-    // (
-    //     n_state: DVCState,
-    //     cid: Slot
-    // )
-    // {
-    //     && cid in n_state.block_consensus_engine_state.active_consensus_instances_on_beacon_blocks 
-    //     ==>
-    //     (
-    //         && cid in n_state.block_consensus_engine_state.block_slashing_db_hist
-    //         && n_state.block_consensus_engine_state.active_consensus_instances_on_beacon_blocks[cid].validityPredicate in n_state.block_consensus_engine_state.block_slashing_db_hist[cid] 
-    //     )
-    // }    
+       
 
-    // predicate inv_current_latest_proposer_duty_match(dv: DVState)    
-    // {
-    //     forall hn |
-    //         && hn in dv.honest_nodes_states.Keys          
-    //         ::
-    //         inv_current_latest_proposer_duty_match_body_body(
-    //             dv.honest_nodes_states[hn]
-    //         )                    
-    // }           
+    predicate inv_current_latest_proposer_duty_match(dv: DVState)    
+    {
+        forall hn |
+            && hn in dv.honest_nodes_states.Keys          
+            ::
+            inv_current_latest_proposer_duty_match_body(
+                dv.honest_nodes_states[hn]
+            )                    
+    }           
 
-    // predicate inv_current_latest_proposer_duty_match_body_body(
-    //     n_state: DVCState
-    // )
-    // {
-    //     (
-    //         && n_state.current_proposer_duty.isPresent()
+    predicate inv_current_latest_proposer_duty_match_body(
+        n_state: DVCState
+    )
+    {
+        (
+            && n_state.current_proposer_duty.isPresent()
             
-    //     ) ==>
-    //     && n_state.latest_proposer_duty.isPresent()
-    //     && n_state.current_proposer_duty.safe_get() == n_state.latest_proposer_duty.safe_get()
-    // }
+        ) ==>
+        && n_state.latest_proposer_duty.isPresent()
+        && n_state.current_proposer_duty.safe_get() == n_state.latest_proposer_duty.safe_get()
+    }
 
     // predicate inv_g_a(dv: DVState)
     // {
@@ -863,64 +1015,64 @@ module Block_Inv_With_Empty_Initial_Block_Slashing_DB
     //             && dv.consensus_instances_on_beacon_block[slot].decided_value.isPresent()
     // }         
 
-    // predicate inv_slot_in_future_decided_data_is_correctody_body(
+    // predicate inv_slot_in_future_beacon_block_is_correctody_body(
     //     dv: DVState, 
     //     n: BLSPubkey,
     //     n_state: DVCState
     // )
     // {
     //     forall slot |
-    //         && slot in n_state.future_proposer_consensus_instances_already_decided
+    //         && slot in n_state.future_consensus_instances_on_blocks_already_decided
     //         ::
     //         dv.consensus_instances_on_beacon_block[slot].decided_value.isPresent()
     // }    
 
-    // predicate inv_rcvd_proposer_duty_is_from_dv_seq_for_rcvd_proposer_duty_body(
-    //     dvc: DVCState,
-    //     hn: BLSPubkey,
-    //     sequence_proposer_duties_to_be_served: iseq<ProposerDutyAndNode>,    
-    //     index_next_proposer_duty_to_be_served: nat
-    // )
-    // {
-    //    forall proposer_duty |
-    //         proposer_duty in dvc.all_rcvd_duties
-    //         ::
-    //         inv_rcvd_proposer_duty_is_from_dv_seq_for_rcvd_proposer_duty_body_body(                
-    //             proposer_duty, 
-    //             hn, 
-    //             sequence_proposer_duties_to_be_served,
-    //             index_next_proposer_duty_to_be_served)
-    // }
+    predicate inv_rcvd_proposer_duty_is_from_dv_seq_for_rcvd_proposer_duty_body(
+        dvc: DVCState,
+        hn: BLSPubkey,
+        sequence_proposer_duties_to_be_served: iseq<ProposerDutyAndNode>,    
+        index_next_proposer_duty_to_be_served: nat
+    )
+    {
+       forall proposer_duty |
+            proposer_duty in dvc.all_rcvd_duties
+            ::
+            inv_rcvd_proposer_duty_is_from_dv_seq_for_rcvd_proposer_duty_body_helper(                
+                proposer_duty, 
+                hn, 
+                sequence_proposer_duties_to_be_served,
+                index_next_proposer_duty_to_be_served)
+    }
 
-    // predicate inv_rcvd_proposer_duty_is_from_dv_seq_for_rcvd_proposer_duty_body_body(        
-    //     proposer_duty: ProposerDuty,
-    //     hn: BLSPubkey, 
-    //     sequence_proposer_duties_to_be_served: iseq<ProposerDutyAndNode>,    
-    //     index_next_proposer_duty_to_be_served: nat
-    // )
-    // {
-    //         exists i ::
-    //             && 0 <= i
-    //             && i < index_next_proposer_duty_to_be_served 
-    //             && var duty_and_node := sequence_proposer_duties_to_be_served[i];
-    //             && duty_and_node.node == hn
-    //             && duty_and_node.proposer_duty == proposer_duty
-    // }
+    predicate inv_rcvd_proposer_duty_is_from_dv_seq_for_rcvd_proposer_duty_body_helper(        
+        proposer_duty: ProposerDuty,
+        hn: BLSPubkey, 
+        sequence_proposer_duties_to_be_served: iseq<ProposerDutyAndNode>,    
+        index_next_proposer_duty_to_be_served: nat
+    )
+    {
+            exists i ::
+                && 0 <= i
+                && i < index_next_proposer_duty_to_be_served 
+                && var duty_and_node := sequence_proposer_duties_to_be_served[i];
+                && duty_and_node.node == hn
+                && duty_and_node.proposer_duty == proposer_duty
+    }
 
-    // predicate inv_rcvd_proposer_duty_is_from_dv_seq_for_rcvd_proposer_duty(dv: DVState)
-    // {
-    //     forall hn: BLSPubkey | 
-    //         is_honest_node(dv, hn) 
-    //         ::
-    //         && var hn_state := dv.honest_nodes_states[hn];
-    //         && inv_rcvd_proposer_duty_is_from_dv_seq_for_rcvd_proposer_duty_body(                    
-    //                 hn_state, 
-    //                 hn, 
-    //                 dv.sequence_proposer_duties_to_be_served,
-    //                 dv.index_next_proposer_duty_to_be_served)
-    // }  
+    predicate inv_rcvd_proposer_duty_is_from_dv_seq_for_rcvd_proposer_duty(dv: DVState)
+    {
+        forall hn: BLSPubkey | 
+            is_honest_node(dv, hn) 
+            ::
+            && var hn_state := dv.honest_nodes_states[hn];
+            && inv_rcvd_proposer_duty_is_from_dv_seq_for_rcvd_proposer_duty_body(                    
+                    hn_state, 
+                    hn, 
+                    dv.sequence_proposer_duties_to_be_served,
+                    dv.index_next_proposer_duty_to_be_served)
+    }  
 
-    // predicate has_all_slashing_db_proposers_before_slot_s(
+    // predicate has_all_slashing_db_blocks_before_slot_s(
     //     db: set<SlashingDBBlock>,
     //     S: set<SlashingDBBlock>,
     //     s: Slot
@@ -929,18 +1081,18 @@ module Block_Inv_With_Empty_Initial_Block_Slashing_DB
     //                 r in db ==> (exists data: BeaconBlock :: r.signing_root == Some(hash_tree_root(data))))
     // {
     //     && S <= db
-    //     && ( forall r | r in db && r !in S :: get_slot_from_slashing_db_proposer(r) >= s )
-    //     && ( forall r | r in S :: get_slot_from_slashing_db_proposer(r) < s )
+    //     && ( forall r | r in db && r !in S :: get_slot_from_slashing_db_block(r) >= s )
+    //     && ( forall r | r in S :: get_slot_from_slashing_db_block(r) < s )
     // }
 
-    // predicate inv_sent_validity_predicate_only_for_slots_stored_in_block_slashing_db_hist(dv: DVState)
-    // {
-    //     forall hn: BLSPubkey, s: Slot | is_honest_node(dv, hn) ::
-    //         && var hn_state := dv.honest_nodes_states[hn];
-    //         && ( hn in dv.consensus_instances_on_beacon_block[s].honest_nodes_validity_functions.Keys
-    //              ==> 
-    //              s in hn_state.block_consensus_engine_state.block_slashing_db_hist.Keys)
-    // }
+    predicate inv_sent_validity_predicate_only_for_slots_stored_in_block_slashing_db_hist(dv: DVState)
+    {
+        forall hn: BLSPubkey, s: Slot | is_honest_node(dv, hn) ::
+            && var hn_state := dv.honest_nodes_states[hn];
+            && ( hn in dv.consensus_instances_on_beacon_block[s].honest_nodes_validity_functions.Keys
+                 ==> 
+                 s in hn_state.block_consensus_engine_state.block_slashing_db_hist.Keys)
+    }
 
     // predicate inv_all_validity_predicates_are_stored_in_block_slashing_db_hist_body(
     //     dv: DVState, 
@@ -951,19 +1103,18 @@ module Block_Inv_With_Empty_Initial_Block_Slashing_DB
     // )
     // requires hn in dv.honest_nodes_states.Keys
     // {
-    //     (
-    //         && var hn_state := dv.honest_nodes_states[hn];
-    //         && hn in dv.consensus_instances_on_beacon_block[s].honest_nodes_validity_functions.Keys
-    //         && s in hn_state.block_consensus_engine_state.block_slashing_db_hist.Keys
-    //         && vp in dv.consensus_instances_on_beacon_block[s].honest_nodes_validity_functions[hn]
-    //     )
+    //     && var hn_state := dv.honest_nodes_states[hn];
+    //     && ((            
+    //             && hn in dv.consensus_instances_on_beacon_block[s].honest_nodes_validity_functions.Keys
+    //             && s in hn_state.block_consensus_engine_state.block_slashing_db_hist.Keys
+    //             && vp in dv.consensus_instances_on_beacon_block[s].honest_nodes_validity_functions[hn]
+    //         )
     //         ==>
-    //     (
-    //         && var hn_state := dv.honest_nodes_states[hn];
-    //         && vp in hn_state.block_consensus_engine_state.block_slashing_db_hist[s]   
-    //     )             
-    // }       
-    
+    //         (
+    //             && vp in hn_state.block_consensus_engine_state.block_slashing_db_hist[s]   
+    //         ))             
+    // }
+
     // predicate inv_all_validity_predicates_are_stored_in_block_slashing_db_hist(dv: DVState)
     // {
     //     forall hn: BLSPubkey, s: Slot, vp : BeaconBlock -> bool |
@@ -976,7 +1127,55 @@ module Block_Inv_With_Empty_Initial_Block_Slashing_DB
     //             s,
     //             vp
     //         )
-    // }              
+    // } 
+
+    predicate inv_all_validity_predicates_are_stored_in_block_slashing_db_hist_body(
+        dv: DVState, 
+        hn: BLSPubkey,
+        hn_state: DVCState,
+        s: Slot,
+        vp: BeaconBlock -> bool
+    )
+    requires && hn in dv.honest_nodes_states.Keys
+             && hn_state == dv.honest_nodes_states[hn]
+             && hn in dv.consensus_instances_on_beacon_block[s].honest_nodes_validity_functions.Keys
+             && s in hn_state.block_consensus_engine_state.block_slashing_db_hist.Keys
+             && vp in dv.consensus_instances_on_beacon_block[s].honest_nodes_validity_functions[hn]
+    {        
+        vp in hn_state.block_consensus_engine_state.block_slashing_db_hist[s]   
+    }
+
+    predicate inv_all_validity_predicates_are_stored_in_block_slashing_db_hist_helper(
+        dv: DVState, 
+        hn: BLSPubkey
+    )
+    requires hn in dv.honest_nodes_states.Keys
+    {
+        && var hn_state := dv.honest_nodes_states[hn];
+        && forall cid: Slot, vp : BeaconBlock -> bool |
+                && hn in dv.consensus_instances_on_beacon_block[cid].honest_nodes_validity_functions.Keys
+                && cid in hn_state.block_consensus_engine_state.block_slashing_db_hist.Keys
+                && vp in dv.consensus_instances_on_beacon_block[cid].honest_nodes_validity_functions[hn]
+                :: 
+                inv_all_validity_predicates_are_stored_in_block_slashing_db_hist_body(
+                    dv,
+                    hn,
+                    dv.honest_nodes_states[hn],
+                    cid,
+                    vp
+                )
+    }       
+    
+    predicate inv_all_validity_predicates_are_stored_in_block_slashing_db_hist(dv: DVState)
+    {
+        forall hn: BLSPubkey |
+            hn in dv.honest_nodes_states.Keys
+            ::
+            inv_all_validity_predicates_are_stored_in_block_slashing_db_hist_helper(
+                dv,
+                hn
+            )
+    }              
 
     // predicate safety(dv: DVState)
     // {
@@ -985,18 +1184,18 @@ module Block_Inv_With_Empty_Initial_Block_Slashing_DB
     //             ==> 
     //             (
     //                 && var S := dv.globally_signed_proposers - { a };
-    //                 && !is_slashable_proposer_data_in_set_of_proposers(S, a.data)
+    //                 && !is_slashable_block_in_set_of_proposers(S, a.data)
     //             )
     // }
 
-    // predicate inv_queued_proposer_duty_is_dvn_seq_of_proposer_duty1<D(!new, 0)>(ci: ConsensusInstance<D>)
+    // predicate inv_queued_proposer_duty_is_dvn_seq_of_proposer_duty1<D(!new, 0)>(ci: BlockConsensusInstance<D>)
     // {
     //     ci.decided_value.isPresent()
     //     <==> 
     //     is_a_valid_decided_value(ci)            
     // }
 
-    // predicate honest_nodes_with_validityPredicate(consa: ConsensusInstance<BeaconBlock>,  h_nodes_a: set<BLSPubkey>)
+    // predicate honest_nodes_with_validityPredicate(consa: BlockConsensusInstance<BeaconBlock>,  h_nodes_a: set<BLSPubkey>)
     // requires h_nodes_a <= consa.honest_nodes_validity_functions.Keys  
     // requires |h_nodes_a| >= quorum(|consa.all_nodes|) 
     //                                     - (|consa.all_nodes| - |consa.honest_nodes_status.Keys|)
@@ -1011,7 +1210,7 @@ module Block_Inv_With_Empty_Initial_Block_Slashing_DB
     //     dv: DVState, 
     //     a: Block, a': Block, 
     //     m: BLSPubkey,
-    //     consa: ConsensusInstance<BeaconBlock>, consa': ConsensusInstance<BeaconBlock>,
+    //     consa: BlockConsensusInstance<BeaconBlock>, consa': BlockConsensusInstance<BeaconBlock>,
     //     h_nodes_a: set<BLSPubkey>, h_nodes_a': set<BLSPubkey>)
     // {
     //     && is_honest_node(dv, m)                
@@ -1026,95 +1225,121 @@ module Block_Inv_With_Empty_Initial_Block_Slashing_DB
     //     && is_a_valid_decided_value_according_to_set_of_nodes(consa', h_nodes_a') 
     // }
 
-    // predicate inv_unique_rcvd_proposer_duty_per_slot(dv: DVState)
-    // {
-    //     forall hn: BLSPubkey | 
-    //         is_honest_node(dv, hn) 
-    //         ::
-    //         inv_unique_rcvd_proposer_duty_per_slot_body(dv.honest_nodes_states[hn])
-    // }
+    predicate inv_unique_rcvd_proposer_duty_per_slot_body_premises(
+        dvc: DVCState,
+        d1: ProposerDuty, 
+        d2: ProposerDuty 
+    )
+    {
+        (   && d1 in dvc.all_rcvd_duties
+            && d2 in dvc.all_rcvd_duties
+            && d1.slot == d2.slot
+        )
+    }
 
-    // predicate inv_unique_rcvd_proposer_duty_per_slot_body(dvc: DVCState)
-    // {
-    //     forall d1: ProposerDuty, d2: ProposerDuty | 
-    //         && d1 in dvc.all_rcvd_duties
-    //         && d2 in dvc.all_rcvd_duties
-    //         && d1.slot == d2.slot
-    //         ::
-    //         d1 == d2
-    // }
+    predicate inv_unique_rcvd_proposer_duty_per_slot_body_helper(
+        dvc: DVCState,
+        d1: ProposerDuty, 
+        d2: ProposerDuty 
+    )
+    {
+        (   && d1 in dvc.all_rcvd_duties
+            && d2 in dvc.all_rcvd_duties
+            && d1.slot == d2.slot
+        )
+        ==>
+        d1 == d2
+    }
 
-    // predicate inv_sent_vp_is_based_on_existing_slashing_db_and_rcvd_proposer_duty_body(
-    //     dv: DVState, 
-    //     hn: BLSPubkey, 
-    //     s: Slot, 
-    //     db: set<SlashingDBBlock>, 
-    //     duty: ProposerDuty, 
-    //     vp: BeaconBlock -> bool)
-    // requires && is_honest_node(dv, hn)
-    //          && var hn_state := dv.honest_nodes_states[hn];
-    //          && s in hn_state.block_consensus_engine_state.block_slashing_db_hist.Keys
-    //          && vp in hn_state.block_consensus_engine_state.block_slashing_db_hist[s]
-    // {
-    //     && var hn_state := dv.honest_nodes_states[hn];
-    //     && duty.slot == s
-    //     && db in hn_state.block_consensus_engine_state.block_slashing_db_hist[s][vp]
-    //     && vp == (ad: BeaconBlock) => ci_decision_ivalilid_beacon_bloc(db, ad, duty)
-    // }
+    predicate inv_unique_rcvd_proposer_duty_per_slot_body(dvc: DVCState)
+    {
+        forall d1: ProposerDuty, d2: ProposerDuty ::
+            ( && d1 in dvc.all_rcvd_duties
+              && d2 in dvc.all_rcvd_duties
+              && d1.slot == d2.slot
+            )
+            ==>
+            d1 == d2
+    }
 
-    // predicate inv_sent_vp_is_based_on_existing_slashing_db_and_rcvd_proposer_duty(dv: DVState)
-    // {
-    //     forall hn: BLSPubkey, s: Slot, vp: BeaconBlock -> bool | 
-    //         && is_honest_node(dv, hn)
-    //         && var hn_state := dv.honest_nodes_states[hn];
-    //         && s in hn_state.block_consensus_engine_state.block_slashing_db_hist.Keys
-    //         && vp in hn_state.block_consensus_engine_state.block_slashing_db_hist[s]
-    //         ::
-    //         exists duty, db ::
-    //             && var hn_state := dv.honest_nodes_states[hn];
-    //             && inv_sent_vp_is_based_on_existing_slashing_db_and_rcvd_proposer_duty_body(dv, hn, s, db, duty, vp)
-    // }
+    predicate inv_unique_rcvd_proposer_duty_per_slot(dv: DVState)
+    {
+        forall hn: BLSPubkey | 
+            is_honest_node(dv, hn) 
+            ::
+            inv_unique_rcvd_proposer_duty_per_slot_body(dv.honest_nodes_states[hn])
+    }
+
+
+
+    predicate inv_sent_vp_is_based_on_existing_slashing_db_and_rcvd_proposer_duty_and_randao_reveal_body(
+        dv: DVState, 
+        hn: BLSPubkey, 
+        s: Slot, 
+        db: set<SlashingDBBlock>, 
+        duty: ProposerDuty, 
+        vp: BeaconBlock -> bool,
+        randao_reveal: BLSSignature
+    )
+    requires && is_honest_node(dv, hn)
+             && var hn_state := dv.honest_nodes_states[hn];
+             && s in hn_state.block_consensus_engine_state.block_slashing_db_hist.Keys
+             && vp in hn_state.block_consensus_engine_state.block_slashing_db_hist[s]
+    {
+        && var hn_state := dv.honest_nodes_states[hn];
+        && duty.slot == s
+        && db in hn_state.block_consensus_engine_state.block_slashing_db_hist[s][vp]
+        && vp == (bb: BeaconBlock) => ci_decision_is_valid_beacon_block(db, bb, duty, randao_reveal)
+    }
+
+    predicate inv_sent_vp_is_based_on_existing_slashing_db_and_rcvd_proposer_duty_and_randao_reveal(dv: DVState)
+    {
+        forall hn: BLSPubkey, s: Slot, vp: BeaconBlock -> bool | 
+            && is_honest_node(dv, hn)
+            && var hn_state := dv.honest_nodes_states[hn];
+            && s in hn_state.block_consensus_engine_state.block_slashing_db_hist.Keys
+            && vp in hn_state.block_consensus_engine_state.block_slashing_db_hist[s]
+            ::
+            exists duty, db, randao_reveal ::
+                && var hn_state := dv.honest_nodes_states[hn];
+                && inv_sent_vp_is_based_on_existing_slashing_db_and_rcvd_proposer_duty_and_randao_reveal_body(dv, hn, s, db, duty, vp, randao_reveal)
+    }
     
-    // predicate inv_decided_data_has_an_honest_witness_body<D(!new, 0)>(ci: ConsensusInstance) 
-    // {
-    //     ci.decided_value.isPresent()
-    //     ==> 
-    //     is_a_valid_decided_value(ci)
-    // }
+    predicate inv_exists_an_honest_dvc_as_a_witness_for_every_decided_beacon_block_body<D(!new, 0)>(ci: BlockConsensusInstance) 
+    {
+        ci.decided_value.isPresent()
+        ==> 
+        is_a_valid_decided_value(ci)
+    }
     
-    // predicate inv_decided_data_has_an_honest_witness(dv: DVState)
-    // {
-    //     forall s: Slot ::
-    //         && var ci := dv.consensus_instances_on_beacon_block[s];
-    //         && inv_decided_data_has_an_honest_witness_body(ci)            
-    // }
+    predicate inv_exists_an_honest_dvc_as_a_witness_for_every_decided_beacon_block(dv: DVState)
+    {
+        forall s: Slot ::
+            && var ci := dv.consensus_instances_on_beacon_block[s];
+            && inv_exists_an_honest_dvc_as_a_witness_for_every_decided_beacon_block_body(ci)            
+    }
 
+    // TODO: prove it
+    predicate inv_proposer_duty_in_next_delivery_is_higher_than_latest_served_proposer_duty_body(dvc: DVCState, next_duty: ProposerDuty)
+    {
+        dvc.latest_proposer_duty.isPresent()
+        ==> 
+        dvc.latest_proposer_duty.safe_get().slot < next_duty.slot        
+    }
 
- 
-    
-
-
-
-    // predicate inv_proposer_duty_in_next_delivery_is_not_lower_than_current_proposer_duty_body(dvc: DVCState, next_duty: ProposerDuty)
-    // {
-    //     dvc.current_proposer_duty.isPresent()
-    //     ==> 
-    //     dvc.current_proposer_duty.safe_get().slot <= next_duty.slot        
-    // }
-
-    // predicate inv_proposer_duty_in_next_delivery_is_not_lower_than_current_proposer_duty(dv: DVState)
-    // {
-    //     && var dv_duty_queue := dv.sequence_proposer_duties_to_be_served;
-    //     && var dv_index := dv.index_next_proposer_duty_to_be_served;
-    //     && var next_duty_and_node := dv_duty_queue[dv_index];
-    //     && forall hn: BLSPubkey | 
-    //         && hn in dv.honest_nodes_states.Keys
-    //         && hn == next_duty_and_node.node 
-    //         ::            
-    //         && var dvc := dv.honest_nodes_states[hn];
-    //         && var next_duty := next_duty_and_node.proposer_duty;
-    //         && inv_proposer_duty_in_next_delivery_is_not_lower_than_current_proposer_duty_body(dvc, next_duty)
-    // }
+    predicate inv_proposer_duty_in_next_delivery_is_higher_than_latest_served_proposer_duty(dv: DVState)
+    {
+        && var dv_duty_queue := dv.sequence_proposer_duties_to_be_served;
+        && var dv_index := dv.index_next_proposer_duty_to_be_served;
+        && var next_duty_and_node := dv_duty_queue[dv_index];
+        && forall hn: BLSPubkey | 
+            && hn in dv.honest_nodes_states.Keys
+            && hn == next_duty_and_node.node 
+            ::            
+            && var dvc := dv.honest_nodes_states[hn];
+            && var next_duty := next_duty_and_node.proposer_duty;
+            && inv_proposer_duty_in_next_delivery_is_higher_than_latest_served_proposer_duty_body(dvc, next_duty)
+    }
 
     // predicate inv_proposer_duty_in_next_delivery_is_not_lower_than_latest_served_proposer_duty_body(dvc: DVCState, next_duty: ProposerDuty)
     // {
@@ -1144,191 +1369,101 @@ module Block_Inv_With_Empty_Initial_Block_Slashing_DB
 
 
 
-    // predicate inv_block_shares_to_broadcast_is_a_subset_of_all_messages_sent_single_node(
-    //     dv: DVState,
-    //     n: BLSPubkey
-    // )
-    // requires n in dv.honest_nodes_states.Keys 
-    // {
-    //     dv.honest_nodes_states[n].block_shares_to_broadcast.Values <= dv.block_share_network.allMessagesSent
-    // }
-
-    // predicate inv_block_shares_to_broadcast_is_a_subset_of_all_messages_sent(
-    //     dv: DVState
-    // )
-    // {
-    //     forall n |
-    //         n in dv.honest_nodes_states.Keys 
-    //         ::
-    //     inv_block_shares_to_broadcast_is_a_subset_of_all_messages_sent_single_node(dv, n)
-    // }    
+  
 
 
-    // predicate inv_active_consensus_instances_implied_the_delivery_of_proposer_duties_body(hn_state: DVCState, s: Slot)
-    // requires s in hn_state.block_consensus_engine_state.block_slashing_db_hist.Keys
-    // {
-    //     exists duty: ProposerDuty :: 
-    //                 && duty in hn_state.all_rcvd_duties
-    //                 && duty.slot == s
-    // }
+    predicate inv_active_consensus_instances_implied_the_delivery_of_proposer_duties_body(hn_state: DVCState, s: Slot)
+    requires s in hn_state.block_consensus_engine_state.block_slashing_db_hist.Keys
+    {
+        exists duty: ProposerDuty :: 
+                    && duty in hn_state.all_rcvd_duties
+                    && duty.slot == s
+    }
 
 
-    // predicate inv_active_consensus_instances_implied_the_delivery_of_proposer_duties(dv: DVState)
-    // {
-    //     forall hn: BLSPubkey, s: Slot ::
-    //         ( && is_honest_node(dv, hn) 
-    //           && var hn_state := dv.honest_nodes_states[hn];
-    //           && s in hn_state.block_consensus_engine_state.block_slashing_db_hist.Keys
-    //         )
-    //         ==>
-    //         inv_active_consensus_instances_implied_the_delivery_of_proposer_duties_body(dv.honest_nodes_states[hn], s)                
-    // }
+    predicate inv_active_consensus_instances_implied_the_delivery_of_proposer_duties(dv: DVState)
+    {
+        forall hn: BLSPubkey, s: Slot ::
+            ( && is_honest_node(dv, hn) 
+              && var hn_state := dv.honest_nodes_states[hn];
+              && s in hn_state.block_consensus_engine_state.block_slashing_db_hist.Keys
+            )
+            ==>
+            inv_active_consensus_instances_implied_the_delivery_of_proposer_duties_body(dv.honest_nodes_states[hn], s)                
+    }
 
-    // predicate inv_block_slashing_db_hist_keeps_track_of_only_rcvd_proposer_duties_body(hn_state: DVCState)    
-    // {
-    //     forall k: Slot | k in hn_state.block_consensus_engine_state.block_slashing_db_hist.Keys ::
-    //         exists duty: ProposerDuty :: 
-    //                 && duty in hn_state.all_rcvd_duties
-    //                 && duty.slot == k
-    // }
 
-    // predicate inv_block_slashing_db_hist_keeps_track_of_only_rcvd_proposer_duties(dv: DVState)
-    // {
-    //     forall hn: BLSPubkey | is_honest_node(dv, hn) ::
-    //         && var hn_state := dv.honest_nodes_states[hn];            
-    //         && inv_block_slashing_db_hist_keeps_track_of_only_rcvd_proposer_duties_body(hn_state)       
-    // }
 
-    // predicate inv_exists_db_in_block_slashing_db_hist_and_duty_for_every_validity_predicate_body_ces(ces: ConsensusEngineState)
-    // {
-    //     forall s: Slot, vp: BeaconBlock -> bool |
-    //             ( && s in ces.block_slashing_db_hist.Keys
-    //               && vp in ces.block_slashing_db_hist[s]
-    //             )
-    //             :: 
-    //             ( exists db: set<SlashingDBBlock>, duty: ProposerDuty ::
-    //                     && duty.slot == s
-    //                     && db in ces.block_slashing_db_hist[s][vp]
-    //                     && vp == (ad: BeaconBlock) => ci_decision_ivalilid_beacon_bloc(db, ad, duty)
-    //             )
-    // }
 
-    // predicate inv_exists_db_in_block_slashing_db_hist_and_duty_for_every_validity_predicate_body(hn_state: DVCState)
-    // {
-    //     forall s: Slot, vp: BeaconBlock -> bool |
-    //             ( && s in hn_state.block_consensus_engine_state.block_slashing_db_hist.Keys
-    //               && vp in hn_state.block_consensus_engine_state.block_slashing_db_hist[s]
-    //             )
-    //             :: 
-    //             ( exists db: set<SlashingDBBlock>, duty: ProposerDuty ::
-    //                     && duty.slot == s
-    //                     && db in hn_state.block_consensus_engine_state.block_slashing_db_hist[s][vp]
-    //                     && vp == (ad: BeaconBlock) => ci_decision_ivalilid_beacon_bloc(db, ad, duty)
-    //             )
-    // }
 
-    // predicate inv_exists_db_in_block_slashing_db_hist_and_duty_for_every_validity_predicate(dv: DVState)
-    // {
-    //     forall hn: BLSPubkey | is_honest_node(dv, hn) ::
-    //         && var dvc := dv.honest_nodes_states[hn];
-    //         && inv_exists_db_in_block_slashing_db_hist_and_duty_for_every_validity_predicate_body(dvc)
-    // }
+    
 
-    // predicate inv_current_validity_predicate_for_slot_k_is_stored_in_block_slashing_db_hist_k_body(hn_state: DVCState)
-    // {
-    //     forall k: Slot |
-    //         k in hn_state.block_consensus_engine_state.active_consensus_instances_on_beacon_blocks.Keys ::
-    //             && var ci := hn_state.block_consensus_engine_state.active_consensus_instances_on_beacon_blocks[k];
-    //             && var vp: BeaconBlock -> bool := ci.validityPredicate;
-    //             && k in hn_state.block_consensus_engine_state.block_slashing_db_hist.Keys 
-    //             && vp in hn_state.block_consensus_engine_state.block_slashing_db_hist[k].Keys             
-    // }
+    predicate inv_monotonic_block_slashing_db_body(dvc: DVCState, dvc': DVCState)
+    {
+        dvc.block_slashing_db <= dvc'.block_slashing_db
+    }
 
-    // predicate inv_current_validity_predicate_for_slot_k_is_stored_in_block_slashing_db_hist_k(dv: DVState)
-    // {
-    //     forall hn: BLSPubkey | is_honest_node(dv, hn) ::
-    //         && var dvc := dv.honest_nodes_states[hn];
-    //         && inv_current_validity_predicate_for_slot_k_is_stored_in_block_slashing_db_hist_k_body(dvc)
-    // }
+    predicate inv_monotonic_block_slashing_db(dv: DVState, event: DV_Block_Proposer_Spec.Event, dv': DVState)    
+    {
+        forall hn: BLSPubkey | is_honest_node(dv, hn) ::
+            && hn in dv'.honest_nodes_states
+            && var dvc := dv.honest_nodes_states[hn];
+            && var dvc' := dv'.honest_nodes_states[hn];
+            && inv_monotonic_block_slashing_db_body(dvc, dvc')
+    }
 
-    // predicate inv_monotonic_block_slashing_db_body(dvc: DVCState, dvc': DVCState)
-    // {
-    //     dvc.block_slashing_db <= dvc'.block_slashing_db
-    // }
+    
+    predicate inv_unchanged_rs_body(dvc: DVCState, dvc': DVCState)
+    {
+        dvc.rs.pubkey == dvc'.rs.pubkey
+    }
 
-    // predicate inv_monotonic_block_slashing_db(dv: DVState, event: DV.Event, dv': DVState)    
-    // {
-    //     forall hn: BLSPubkey | is_honest_node(dv, hn) ::
-    //         && hn in dv'.honest_nodes_states
-    //         && var dvc := dv.honest_nodes_states[hn];
-    //         && var dvc' := dv'.honest_nodes_states[hn];
-    //         && inv_monotonic_block_slashing_db_body(dvc, dvc')
-    // }
-
-    // predicate inv_every_db_in_block_slashing_db_hist_is_subset_of_block_slashing_db_body_ces(ces: ConsensusEngineState, block_slashing_db: set<SlashingDBBlock>)
-    // {
-    //     forall s: Slot, vp: BeaconBlock -> bool, db: set<SlashingDBBlock> |
-    //             ( && s in ces.block_slashing_db_hist.Keys
-    //               && vp in ces.block_slashing_db_hist[s]
-    //               && db in ces.block_slashing_db_hist[s][vp]
-    //             )
-    //             :: 
-    //             db <= block_slashing_db
-    // }
-
-    // predicate inv_every_db_in_block_slashing_db_hist_is_subset_of_block_slashing_db_body(hn_state: DVCState)
-    // {
-    //     forall s: Slot, vp: BeaconBlock -> bool, db: set<SlashingDBBlock> |
-    //             ( && s in hn_state.block_consensus_engine_state.block_slashing_db_hist.Keys
-    //               && vp in hn_state.block_consensus_engine_state.block_slashing_db_hist[s]
-    //               && db in hn_state.block_consensus_engine_state.block_slashing_db_hist[s][vp]
-    //             )
-    //             :: 
-    //             db <= hn_state.block_slashing_db
-    // }
-
-    // predicate inv_every_db_in_block_slashing_db_hist_is_subset_of_block_slashing_db(dv: DVState)
-    // {
-    //     forall hn: BLSPubkey | is_honest_node(dv, hn) ::
-    //         && var dvc := dv.honest_nodes_states[hn];
-    //         && inv_every_db_in_block_slashing_db_hist_is_subset_of_block_slashing_db_body(dvc)
-    // }
-
-    // predicate inv_monotonic_block_slashing_db_hist_body(dvc: DVCState, dvc': DVCState)
-    // {        
-    //     dvc.block_consensus_engine_state.block_slashing_db_hist.Keys
-    //     <= 
-    //     dvc'.block_consensus_engine_state.block_slashing_db_hist.Keys
-    // }
-
-    // predicate inv_monotonic_block_slashing_db_hist(dv: DVState, event: DV.Event, dv': DVState)    
-    // {
-    //     forall hn: BLSPubkey | is_honest_node(dv, hn) ::
-    //         && hn in dv'.honest_nodes_states
-    //         && var dvc := dv.honest_nodes_states[hn];
-    //         && var dvc' := dv'.honest_nodes_states[hn];
-    //         && inv_monotonic_block_slashing_db_hist_body(dvc, dvc')
-    // }
 
     // predicate prop_monotonic_set_of_in_transit_messages(dv: DVState, dv': DVState)
     // {
     //     && dv.block_share_network.allMessagesSent <= dv'.block_share_network.allMessagesSent
     // }
-     
-   
-    // predicate inv_active_proposern_consensus_instances_are_tracked_in_block_slashing_db_hist_body(dvc: DVCState)
-    // {
-    //     dvc.block_consensus_engine_state.active_consensus_instances_on_beacon_blocks.Keys 
-    //     <= 
-    //     dvc.block_consensus_engine_state.block_slashing_db_hist.Keys
-    // } 
 
-    // predicate inv_active_proposern_consensus_instances_are_tracked_in_block_slashing_db_hist(dv: DVState)
-    // {
-    //     forall hn | hn in dv.honest_nodes_states.Keys ::
-    //         && var dvc := dv.honest_nodes_states[hn];
-    //         && inv_active_proposern_consensus_instances_are_tracked_in_block_slashing_db_hist_body(dvc)
-    // } 
+
+
+    predicate inv_constraints_on_active_consensus_instances_on_beacon_blocks_are_ensured_with_block_slashing_db_hist(dv: DVState)    
+    {
+        forall hn, cid |
+            && hn in dv.honest_nodes_states.Keys        
+            ::
+            inv_constraints_on_active_consensus_instances_on_beacon_blocks_are_ensured_with_block_slashing_db_hist_body(dv.honest_nodes_states[hn], cid)
+             
+    }       
+
+    predicate inv_constraints_on_active_consensus_instances_on_beacon_blocks_are_ensured_with_block_slashing_db_hist_body
+    (
+        n_state: DVCState,
+        cid: Slot
+    )
+    {
+        && cid in n_state.block_consensus_engine_state.active_consensus_instances_on_beacon_blocks.Keys 
+        ==>
+        (
+            // can imply from inv_active_consensus_instances_on_beacon_blocks_are_tracked_in_block_slashing_db_hist_body
+            && cid in n_state.block_consensus_engine_state.block_slashing_db_hist.Keys  
+            // check that inv_active_attestation_consensus_instances_keys_is_subset_of_att_slashing_db_hist_body_body
+            && n_state.block_consensus_engine_state.active_consensus_instances_on_beacon_blocks[cid].validityPredicate in n_state.block_consensus_engine_state.block_slashing_db_hist[cid] 
+        )
+    }  
+   
+    predicate inv_active_consensus_instances_on_beacon_blocks_are_tracked_in_block_slashing_db_hist_body(dvc: DVCState)
+    {
+        dvc.block_consensus_engine_state.active_consensus_instances_on_beacon_blocks.Keys 
+        <= 
+        dvc.block_consensus_engine_state.block_slashing_db_hist.Keys
+    } 
+
+    predicate inv_active_consensus_instances_on_beacon_blocks_are_tracked_in_block_slashing_db_hist(dv: DVState)
+    {
+        forall hn | hn in dv.honest_nodes_states.Keys ::
+            && var dvc := dv.honest_nodes_states[hn];
+            && inv_active_consensus_instances_on_beacon_blocks_are_tracked_in_block_slashing_db_hist_body(dvc)
+    } 
 
     // predicate inv_construct_complete_signed_signature_assumptions_helper(dv: DVState)
     // {
@@ -1340,48 +1475,11 @@ module Block_Inv_With_Empty_Initial_Block_Slashing_DB
 
 
 
-    // predicate inv_rcvd_proposern_shares_are_from_sent_messages_body(
-    //     dv: DVState,
-    //     dvc: DVCState
-    // )
-    // {
-    //     var rcvd_block_shares := dvc.rcvd_block_shares;
-
-    //     forall i, j |
-    //         && i in rcvd_block_shares.Keys 
-    //         && j in rcvd_block_shares[i]
-    //         ::
-    //         rcvd_block_shares[i][j] <= dv.block_share_network.allMessagesSent
-    // }    
-
-    // predicate inv_rcvd_proposern_shares_are_from_sent_messages(
-    //     dv: DVState    
-    // )
-    // {
-    //     forall n | n in dv.honest_nodes_states ::
-    //         && var dvc := dv.honest_nodes_states[n];
-    //         && inv_rcvd_proposern_shares_are_from_sent_messages_body(dv, dvc)
-    // } 
 
 
-    // predicate inv_block_shares_to_broadcast_are_sent_messages_body(
-    //     dv: DVState,
-    //     dvc: DVCState
-    // )    
-    // {
-    //     dvc.block_shares_to_broadcast.Values <= dv.block_share_network.allMessagesSent
-    // }
 
-    // predicate inv_block_shares_to_broadcast_are_sent_messages(
-    //     dv: DVState
-    // )
-    // {
-    //     forall n | n in dv.honest_nodes_states.Keys ::
-    //         && var dvc := dv.honest_nodes_states[n];
-    //         && inv_block_shares_to_broadcast_are_sent_messages_body(dv, dvc)
-    // }
 
-    // predicate inv39(
+    // predicate inv_monotonic_block_share_network(
     //     dv: DVState,        
     //     dv': DVState
     // )       
@@ -1390,37 +1488,25 @@ module Block_Inv_With_Empty_Initial_Block_Slashing_DB
     // }
 
     
-    // predicate inv_slots_for_sent_validity_predicate_are_stored_in_block_slashing_db_hist_body(
-    //     dv: DVState, 
-    //     hn: BLSPubkey,
-    //     hn_state: DVCState,
-    //     s: Slot
-    // )
-    // {
-    //     hn in dv.consensus_instances_on_beacon_block[s].honest_nodes_validity_functions.Keys
-    //     ==> s in hn_state.block_consensus_engine_state.block_slashing_db_hist.Keys
-    // }
+    predicate inv_slots_for_sent_validity_predicate_are_stored_in_block_slashing_db_hist_body(
+        dv: DVState, 
+        hn: BLSPubkey,
+        hn_state: DVCState,
+        s: Slot
+    )
+    {
+        hn in dv.consensus_instances_on_beacon_block[s].honest_nodes_validity_functions.Keys
+        ==> 
+        s in hn_state.block_consensus_engine_state.block_slashing_db_hist.Keys
+    }
 
-    // predicate inv_slots_for_sent_validity_predicate_are_stored_in_block_slashing_db_hist(dv: DVState)
-    // {
-    //     forall hn: BLSPubkey, s: Slot |
-    //         hn in dv.honest_nodes_states
-    //         :: 
-    //         inv_slots_for_sent_validity_predicate_are_stored_in_block_slashing_db_hist_body(dv, hn, dv.honest_nodes_states[hn], s)        
-    // } 
-
-    // predicate inv_no_active_consensus_instance_before_receiving_proposer_duty_body(dvc: DVCState)
-    // {
-    //     !dvc.latest_proposer_duty.isPresent()
-    //     ==> dvc.block_consensus_engine_state.active_consensus_instances_on_beacon_blocks.Keys == {}
-    // }
-
-    // predicate inv_no_active_consensus_instance_before_receiving_proposer_duty(dv: DVState)
-    // {
-    //     forall hn: BLSPubkey | hn in dv.honest_nodes_states.Keys ::
-    //         && var dvc := dv.honest_nodes_states[hn];
-    //         && inv_no_active_consensus_instance_before_receiving_proposer_duty_body(dvc)
-    // }
+    predicate inv_slots_for_sent_validity_predicate_are_stored_in_block_slashing_db_hist(dv: DVState)
+    {
+        forall hn: BLSPubkey, s: Slot |
+            hn in dv.honest_nodes_states
+            :: 
+            inv_slots_for_sent_validity_predicate_are_stored_in_block_slashing_db_hist_body(dv, hn, dv.honest_nodes_states[hn], s)        
+    } 
 
     // predicate inv_slot_of_active_consensus_instance_is_lower_than_slot_of_latest_served_proposer_duty_body(dvc: DVCState)
     // {
@@ -1438,67 +1524,66 @@ module Block_Inv_With_Empty_Initial_Block_Slashing_DB
     //         && inv_slot_of_active_consensus_instance_is_lower_than_slot_of_latest_served_proposer_duty_body(dvc)
     // }
 
-    // predicate inv_consensus_instances_are_isConditionForSafetyTrue(dv: DVState)
-    // {
-    //     forall slot: Slot | slot in dv.consensus_instances_on_beacon_block.Keys  ::
-    //                 isConditionForSafetyTrue(dv.consensus_instances_on_beacon_block[slot])                    
-    // }
+    predicate inv_consensus_instance_isConditionForSafetyTrue(dv: DVState)
+    {
+        forall slot: Slot | slot in dv.consensus_instances_on_beacon_block.Keys  ::
+                    isConditionForSafetyTrue(dv.consensus_instances_on_beacon_block[slot])                    
+    }
 
-    // predicate pred_last_proposer_duty_is_delivering_to_given_honest_node(
-    //     proposer_duty: ProposerDuty,
-    //     dv: DVState,
-    //     n: BLSPubkey,
-    //     index_next_proposer_duty_to_be_served: nat
-    // )
-    // {
-    //     && 0 < index_next_proposer_duty_to_be_served 
-    //     && var i := index_next_proposer_duty_to_be_served - 1;
-    //     && var an := dv.sequence_proposer_duties_to_be_served[i];
-    //     && an.proposer_duty == proposer_duty
-    //     && an.node == n
-    // }
+    predicate pred_last_proposer_duty_is_delivering_to_given_honest_node(
+        proposer_duty: ProposerDuty,
+        sequence_proposer_duties_to_be_served: iseq<ProposerDutyAndNode>,
+        n: BLSPubkey,
+        index_next_proposer_duty_to_be_served: nat
+    )
+    {
+        && 0 < index_next_proposer_duty_to_be_served 
+        && var i := index_next_proposer_duty_to_be_served - 1;
+        && var pn := sequence_proposer_duties_to_be_served[i];
+        && pn.proposer_duty == proposer_duty
+        && pn.node == n
+    }
 
-    // predicate inv_none_latest_proposer_duty_and_empty_set_of_rcvd_proposer_duties_body(dvc: DVCState)
-    // {
-    //     !dvc.latest_proposer_duty.isPresent()
-    //     <==> 
-    //     dvc.all_rcvd_duties == {}
-    // }
+    predicate inv_none_latest_proposer_duty_and_empty_set_of_rcvd_proposer_duties_body(dvc: DVCState)
+    {
+        !dvc.latest_proposer_duty.isPresent()
+        <==> 
+        dvc.all_rcvd_duties == {}
+    }
 
-    // predicate inv_none_latest_proposer_duty_and_empty_set_of_rcvd_proposer_duties(dv: DVState)
-    // {
-    //     forall hn: BLSPubkey | hn in dv.honest_nodes_states.Keys ::
-    //         inv_none_latest_proposer_duty_and_empty_set_of_rcvd_proposer_duties_body(dv.honest_nodes_states[hn])
-    // }
+    predicate inv_none_latest_proposer_duty_and_empty_set_of_rcvd_proposer_duties(dv: DVState)
+    {
+        forall hn: BLSPubkey | hn in dv.honest_nodes_states.Keys ::
+            inv_none_latest_proposer_duty_and_empty_set_of_rcvd_proposer_duties_body(dv.honest_nodes_states[hn])
+    }
 
-    // predicate inv_no_rcvd_proposer_duty_is_higher_than_latest_proposer_duty_body(dvc: DVCState)
-    // {
-    //     dvc.latest_proposer_duty.isPresent()
-    //     ==>
-    //     ( forall proposer_duty | proposer_duty in dvc.all_rcvd_duties ::
-    //         proposer_duty.slot <= dvc.latest_proposer_duty.safe_get().slot
-    //     )
-    // }
+    predicate inv_no_rcvd_proposer_duty_is_higher_than_latest_proposer_duty_body(dvc: DVCState)
+    {
+        dvc.latest_proposer_duty.isPresent()
+        ==>
+        ( forall proposer_duty | proposer_duty in dvc.all_rcvd_duties ::
+            proposer_duty.slot <= dvc.latest_proposer_duty.safe_get().slot
+        )
+    }
 
-    // predicate inv_no_rcvd_proposer_duty_is_higher_than_latest_proposer_duty(dv: DVState)
-    // {
-    //     forall hn: BLSPubkey | hn in dv.honest_nodes_states.Keys ::
-    //         &&  var dvc := dv.honest_nodes_states[hn];
-    //         &&  inv_no_rcvd_proposer_duty_is_higher_than_latest_proposer_duty_body(dvc)
-    // }
-
-    // predicate inv_data_of_all_created_proposers_is_set_of_decided_values(dv: DVState)
-    // {
-    //     forall a | a in dv.all_proposers_created ::
-    //             && var consa := dv.consensus_instances_on_beacon_block[a.data.slot];
-    //             && consa.decided_value.isPresent() 
-    //             && a.data == consa.decided_value.safe_get() 
-    // }
+    predicate inv_no_rcvd_proposer_duty_is_higher_than_latest_proposer_duty(dv: DVState)
+    {
+        forall hn: BLSPubkey | hn in dv.honest_nodes_states.Keys ::
+            &&  var dvc := dv.honest_nodes_states[hn];
+            &&  inv_no_rcvd_proposer_duty_is_higher_than_latest_proposer_duty_body(dvc)
+    }
+    predicate inv_block_of_all_created_blocks_is_set_of_decided_values(dv: DVState)
+    {
+        forall complete_block | complete_block in dv.all_blocks_created ::
+                && var consa := dv.consensus_instances_on_beacon_block[complete_block.block.slot];
+                && consa.decided_value.isPresent() 
+                && complete_block.block == consa.decided_value.safe_get() 
+    }
 
     // predicate inv_one_honest_dvc_is_required_to_pass_signer_threshold(
     //     dv: DVState,
     //     signers: set<BLSPubkey>,
-    //     block_shares: set<BlockShare>,
+    //     block_shares: set<SignedBeaconBlock>,
     //     signing_root: Root
     // )
     // {
@@ -1514,21 +1599,21 @@ module Block_Inv_With_Empty_Initial_Block_Slashing_DB
     //     )
     // }
 
-    // predicate inv_all_created_proposers_are_valid(dv: DVState)
-    // {
-    //     forall a | a in dv.all_proposers_created ::
-    //             is_valid_proposer(a, dv.dv_pubkey)
-    // }
+    predicate inv_all_created_signed_beacon_blocks_are_valid(dv: DVState)
+    {
+        forall b | b in dv.all_blocks_created ::
+                is_valid_signed_beacon_block(b, dv.dv_pubkey)
+    }
 
-    // predicate inv_outputs_proposers_submited_are_valid(
-    //     outputs: Outputs,
-    //     dv_pubkey: BLSPubkey)
-    // {
-    //     forall submitted_block | submitted_block in outputs.proposers_submitted ::
-    //         is_valid_proposer(submitted_block, dv_pubkey)
-    // }
+    predicate inv_submitted_outputs_blocks_are_valid(
+        outputs: Outputs,
+        dv_pubkey: BLSPubkey)
+    {
+        forall submitted_block | submitted_block in outputs.submitted_blocks ::
+            is_valid_signed_beacon_block(submitted_block, dv_pubkey)
+    }
 
-    // predicate pred_slashing_db_proposer_in_two_dbs(
+    // predicate pred_slashing_db_block_in_two_dbs(
     //     sdba: SlashingDBBlock,
     //     db1: set<SlashingDBBlock>,
     //     db2: set<SlashingDBBlock>
@@ -1538,7 +1623,7 @@ module Block_Inv_With_Empty_Initial_Block_Slashing_DB
     //     && sdba in db2
     // }
 
-    // predicate inv_slashing_db_proposer_in_db_for_low_slot_is_in_db_for_high_slot_body_helper(
+    // predicate inv_slashing_db_block_in_db_for_low_slot_is_in_db_for_high_slot_body_helper(
     //             set_db:  set<set<SlashingDBBlock>>,
     //             set_db':  set<set<SlashingDBBlock>>
     // )
@@ -1553,7 +1638,7 @@ module Block_Inv_With_Empty_Initial_Block_Slashing_DB
     //         )
     // }
 
-    // predicate inv_slashing_db_proposer_in_db_for_low_slot_is_in_db_for_high_slot_body_body(
+    // predicate inv_slashing_db_block_in_db_for_low_slot_is_in_db_for_high_slot_body(
     //     db_hist_on_slot: map<BeaconBlock -> bool, set<set<SlashingDBBlock>>>,
     //     db_hist_on_slot': map<BeaconBlock -> bool, set<set<SlashingDBBlock>>>
     // )
@@ -1562,14 +1647,14 @@ module Block_Inv_With_Empty_Initial_Block_Slashing_DB
     //         && vp in db_hist_on_slot.Keys
     //         && vp' in db_hist_on_slot'.Keys 
     //         ::
-    //         inv_slashing_db_proposer_in_db_for_low_slot_is_in_db_for_high_slot_body_helper(
+    //         inv_slashing_db_block_in_db_for_low_slot_is_in_db_for_high_slot_body_helper(
     //             db_hist_on_slot[vp],
     //             db_hist_on_slot'[vp']
     //         )
              
     // }
 
-    // predicate inv_slashing_db_proposer_in_db_for_low_slot_is_in_db_for_high_slot_body(
+    // predicate inv_slashing_db_block_in_db_for_low_slot_is_in_db_for_high_slot_body(
     //     dvc: DVCState
     // )
     // {
@@ -1578,35 +1663,34 @@ module Block_Inv_With_Empty_Initial_Block_Slashing_DB
     //         && slot' in dvc.block_consensus_engine_state.block_slashing_db_hist.Keys 
     //         && slot < slot'
     //         ::
-    //         inv_slashing_db_proposer_in_db_for_low_slot_is_in_db_for_high_slot_body_body(
+    //         inv_slashing_db_block_in_db_for_low_slot_is_in_db_for_high_slot_body(
     //              dvc.block_consensus_engine_state.block_slashing_db_hist[slot], 
     //              dvc.block_consensus_engine_state.block_slashing_db_hist[slot']
     //         )
     // }
 
-    // predicate inv_slashing_db_proposer_in_db_for_low_slot_is_in_db_for_high_slot(
+    // predicate inv_slashing_db_block_in_db_for_low_slot_is_in_db_for_high_slot(
     //     dv: DVState
     // )
     // {
     //     forall hn: BLSPubkey | is_honest_node(dv, hn) ::
-    //         inv_slashing_db_proposer_in_db_for_low_slot_is_in_db_for_high_slot_body(dv.honest_nodes_states[hn])
+    //         inv_slashing_db_block_in_db_for_low_slot_is_in_db_for_high_slot_body(dv.honest_nodes_states[hn])
         
     // }
 
-    // predicate pred_verify_owner_of_block_share_with_bls_signature(
-    //     rs_pubkey: BLSPubkey,
-    //     block_share: SignedBeaconBlock
-    // )
-    // {
-    //     && var decided_beacon_block := block_share.block;
-    //     && var fork_version := bn_get_fork_version(compute_start_slot_at_epoch(decided_beacon_block.target.epoch));
-    //     && var proposer_signing_root := compute_proposer_signing_root(decided_beacon_block, fork_version);
-    //     && verify_bls_signature(proposer_signing_root, block_share.signature, rs_pubkey)
-    // }
+    predicate pred_verify_owner_of_block_share_with_bls_signature(
+        rs_pubkey: BLSPubkey,
+        block_share: SignedBeaconBlock
+    )
+    {
+        && var decided_beacon_block := block_share.block;
+        && var block_signing_root := compute_block_signing_root(decided_beacon_block);
+        && verify_bls_signature(block_signing_root, block_share.signature, rs_pubkey)
+    }
 
     // predicate pred_is_owner_of_one_proposerestaion_share_in_set_of_shares(
     //     rs_pubkey: BLSPubkey,
-    //     block_shares: set<BlockShare>
+    //     block_shares: set<SignedBeaconBlock>
     // )
     // {
     //     exists share | share in block_shares ::
@@ -1615,15 +1699,15 @@ module Block_Inv_With_Empty_Initial_Block_Slashing_DB
 
     // predicate pred_proposer_is_created_based_on_sent_block_shares(
     //     dv: DVState,
-    //     proposer: Block,
-    //     block_shares: set<BlockShare>
+    //     block: SignedBeaconBlock,
+    //     block_shares: set<SignedBeaconBlock>
     // )
     // {
     //     && block_shares <= dv.block_share_network.allMessagesSent
     //     && var constructed_sig := dv.construct_complete_signed_block(block_shares);
     //     && constructed_sig.isPresent()
     //     && constructed_sig.safe_get() == proposer.signature
-    //     && all_block_shares_have_the_same_data(block_shares, proposer.data)
+    //     && signed_beacon_blocks_for_the_same_beacon_block(block_shares, block.block)
     // }
 
     // predicate inv_exists_honest_node_that_contributed_to_creation_of_two_submitted_blocks_body(
@@ -1632,7 +1716,7 @@ module Block_Inv_With_Empty_Initial_Block_Slashing_DB
     //     a': Block
     // )
     // {
-    //     exists hn: BLSPubkey, block_shares: set<BlockShare>, block_shares': set<BlockShare> ::
+    //     exists hn: BLSPubkey, block_shares: set<SignedBeaconBlock>, block_shares': set<SignedBeaconBlock> ::
     //         && is_honest_node(dv, hn)
     //         && var rs_pubkey: BLSPubkey := dv.honest_nodes_states[hn].rs.pubkey;
     //         && pred_proposer_is_created_based_on_sent_block_shares(dv, a, block_shares)            
@@ -1645,33 +1729,33 @@ module Block_Inv_With_Empty_Initial_Block_Slashing_DB
     //     dv: DVState)
     // {
     //     forall a: Block, a': Block |
-    //         && a in dv.all_proposers_created
-    //         && a' in dv.all_proposers_created
+    //         && a in dv.all_blocks_created
+    //         && a' in dv.all_blocks_created
     //         ::
     //         inv_exists_honest_node_that_contributed_to_creation_of_two_submitted_blocks_body(dv, a, a')
     // }
     
-    // predicate inv_if_honest_node_sends_block_share_it_receives_proposer_data_before_body(
+    // predicate inv_if_honest_node_sends_block_share_it_receives_beacon_block_before_body(
     //     dvc: DVCState,
     //     block_share: SignedBeaconBlock
     // )
     // {
-    //     && var proposer_data: BeaconBlock := block_share.block;
-    //     && var slot: Slot := proposer_data.slot;
-    //     && var slashing_db_proposer := SlashingDBBlock(
-    //                                         source_epoch := proposer_data.source.epoch,
-    //                                         target_epoch := proposer_data.target.epoch,
-    //                                         signing_root := Some(hash_tree_root(proposer_data)));
-    //     && slashing_db_proposer in dvc.block_slashing_db
+    //     && var beacon_block: BeaconBlock := block_share.block;
+    //     && var slot: Slot := beacon_block.slot;
+    //     && var slashing_db_block := SlashingDBBlock(
+    //                                         source_epoch := beacon_block.source.epoch,
+    //                                         target_epoch := beacon_block.target.epoch,
+    //                                         signing_root := Some(hash_tree_root(beacon_block)));
+    //     && slashing_db_block in dvc.block_slashing_db
     //     && exists proposer_duty: ProposerDuty, vp: BeaconBlock -> bool :: 
     //             (   && proposer_duty in dvc.all_rcvd_duties
     //                 && slot in dvc.block_consensus_engine_state.block_slashing_db_hist.Keys
     //                 && vp in dvc.block_consensus_engine_state.block_slashing_db_hist[slot].Keys
-    //                 && vp(proposer_data)
+    //                 && vp(beacon_block)
     //             )
     // }
 
-    // predicate inv_if_honest_node_sends_block_share_it_receives_proposer_data_before(dv: DVState)
+    // predicate inv_if_honest_node_sends_block_share_it_receives_beacon_block_before(dv: DVState)
     // {
     //     forall hn, block_share |
     //         && is_honest_node(dv, hn)
@@ -1680,7 +1764,7 @@ module Block_Inv_With_Empty_Initial_Block_Slashing_DB
     //         && pred_verify_owner_of_block_share_with_bls_signature(rs_pubkey, block_share)
     //         ::
     //         && var dvc := dv.honest_nodes_states[hn];
-    //         && inv_if_honest_node_sends_block_share_it_receives_proposer_data_before_body(dvc, block_share)
+    //         && inv_if_honest_node_sends_block_share_it_receives_beacon_block_before_body(dvc, block_share)
     // }
 
     // predicate inv_data_of_sent_block_shares_is_known_body(
@@ -1688,122 +1772,123 @@ module Block_Inv_With_Empty_Initial_Block_Slashing_DB
     //     block_share: SignedBeaconBlock
     // )
     // {
-    //     && var proposer_data: BeaconBlock := block_share.block;
-    //     && var slot: Slot := proposer_data.slot;
-    //     && var slashing_db_proposer := SlashingDBBlock(
-    //                                         source_epoch := proposer_data.source.epoch,
-    //                                         target_epoch := proposer_data.target.epoch,
-    //                                         signing_root := Some(hash_tree_root(proposer_data)));
-    //     && slashing_db_proposer in dvc.block_slashing_db
+    //     && var beacon_block: BeaconBlock := block_share.block;
+    //     && var slot: Slot := beacon_block.slot;
+    //     && var slashing_db_block := SlashingDBBlock(
+    //                                         source_epoch := beacon_block.source.epoch,
+    //                                         target_epoch := beacon_block.target.epoch,
+    //                                         signing_root := Some(hash_tree_root(beacon_block)));
+    //     && slashing_db_block in dvc.block_slashing_db
     //     && exists proposer_duty: ProposerDuty, vp: BeaconBlock -> bool :: 
     //             (   && proposer_duty in dvc.all_rcvd_duties
     //                 && slot in dvc.block_consensus_engine_state.block_slashing_db_hist.Keys
     //                 && vp in dvc.block_consensus_engine_state.block_slashing_db_hist[slot].Keys
-    //                 && vp(proposer_data)
+    //                 && vp(beacon_block)
     //             )
     // }
 
-    // predicate inv_outputs_block_shares_sent_is_tracked_in_block_slashing_db_body(
-    //     dvc: DVCState, 
-    //     block_share: SignedBeaconBlock
-    // )
-    // {
-    //     && var proposer_data: BeaconBlock := block_share.block;
-    //     && var slashing_db_proposer := construct_SlashingDBBlock_from_proposer_data(proposer_data);
-    //     && slashing_db_proposer in dvc.block_slashing_db  
-    //     && var rs_pubkey: BLSPubkey := dvc.rs.pubkey;    
-    //     && pred_verify_owner_of_block_share_with_bls_signature(rs_pubkey, block_share)
-    // }   
+    predicate inv_outputs_sent_block_shares_is_tracked_in_block_slashing_db_body(
+        dvc: DVCState, 
+        block_share: SignedBeaconBlock
+    )
+    {
+        && var beacon_block: BeaconBlock := block_share.block;
+        && var slashing_db_block := construct_SlashingDBBlock_from_beacon_block(beacon_block);
+        && slashing_db_block in dvc.block_slashing_db  
+        && var rs_pubkey: BLSPubkey := dvc.rs.pubkey;    
+        && pred_verify_owner_of_block_share_with_bls_signature(rs_pubkey, block_share)
+    }   
 
-    // predicate inv_outputs_block_shares_sent_is_tracked_in_block_slashing_db(
-    //     outputs: Outputs,
-    //     dvc: DVCState)
-    // {
-    //     forall block_share: SignedBeaconBlock | 
-    //         block_share in getMessagesFromMessagesWithRecipient(outputs.block_shares_sent) 
-    //         ::
-    //         inv_outputs_block_shares_sent_is_tracked_in_block_slashing_db_body(dvc, block_share)
-    // } 
+                         
+    predicate inv_outputs_sent_block_shares_is_tracked_in_block_slashing_db(
+        outputs: Outputs,
+        dvc: DVCState)
+    {
+        forall block_share: SignedBeaconBlock | 
+            block_share in getMessagesFromMessagesWithRecipient(outputs.sent_block_shares) 
+            ::
+            inv_outputs_sent_block_shares_is_tracked_in_block_slashing_db_body(dvc, block_share)
+    } 
 
-    // predicate inv_block_shares_to_broadcast_is_tracked_in_block_slashing_db_body(
-    //     dvc: DVCState
-    // )
-    // {
-    //     forall slot: Slot | 
-    //         slot in dvc.block_shares_to_broadcast.Keys
-    //         ::
-    //         && var block_share: SignedBeaconBlock := dvc.block_shares_to_broadcast[slot];
-    //         && var proposer_data: BeaconBlock := block_share.block;
-    //         && var slashing_db_proposer := construct_SlashingDBBlock_from_proposer_data(proposer_data);
-    //         && slashing_db_proposer in dvc.block_slashing_db  
-    //         && var rs_pubkey: BLSPubkey := dvc.rs.pubkey;    
-    //         && pred_verify_owner_of_block_share_with_bls_signature(rs_pubkey, block_share)
-    // }   
+    predicate inv_block_shares_to_broadcast_is_tracked_in_block_slashing_db_body(
+        dvc: DVCState
+    )
+    {
+        forall slot: Slot | 
+            slot in dvc.block_shares_to_broadcast.Keys
+            ::
+            && var block_share: SignedBeaconBlock := dvc.block_shares_to_broadcast[slot];
+            && var beacon_block: BeaconBlock := block_share.block;
+            && var slashing_db_block := construct_SlashingDBBlock_from_beacon_block(beacon_block);
+            && slashing_db_block in dvc.block_slashing_db  
+            && var rs_pubkey: BLSPubkey := dvc.rs.pubkey;    
+            && pred_verify_owner_of_block_share_with_bls_signature(rs_pubkey, block_share)
+    }   
 
-    // predicate inv_block_shares_to_broadcast_is_tracked_in_block_slashing_db(
-    //     dv: DVState)
-    // {
-    //     forall hn: BLSPubkey | 
-    //         is_honest_node(dv, hn)
-    //         ::
-    //         inv_block_shares_to_broadcast_is_tracked_in_block_slashing_db_body(dv.honest_nodes_states[hn])
-    // } 
+    predicate inv_block_shares_to_broadcast_is_tracked_in_block_slashing_db(
+        dv: DVState)
+    {
+        forall hn: BLSPubkey | 
+            is_honest_node(dv, hn)
+            ::
+            inv_block_shares_to_broadcast_is_tracked_in_block_slashing_db_body(dv.honest_nodes_states[hn])
+    } 
 
-    // predicate inv_block_of_block_shares_is_known_body(
-    //     dvc: DVCState,
-    //     block_share: SignedBeaconBlock
-    // )
-    // {
-    //     && var proposer_data := block_share.block;
-    //     && var slashing_db_proposer := construct_SlashingDBBlock_from_proposer_data(proposer_data);
-    //     && slashing_db_proposer in dvc.block_slashing_db     
-    // }
+    predicate inv_block_of_block_shares_is_known_body(
+        dvc: DVCState,
+        block_share: SignedBeaconBlock
+    )
+    {
+        && var beacon_block := block_share.block;
+        && var slashing_db_block := construct_SlashingDBBlock_from_beacon_block(beacon_block);
+        && slashing_db_block in dvc.block_slashing_db     
+    }
 
-    // predicate inv_block_of_block_shares_is_known(
-    //     dv: DVState
-    // )
-    // {
-    //     forall hn: BLSPubkey, block_share: SignedBeaconBlock | 
-    //         && is_honest_node(dv, hn)
-    //         && block_share in dv.block_share_network.allMessagesSent 
-    //         && var dvc: DVCState := dv.honest_nodes_states[hn];
-    //         && var rs_pubkey: BLSPubkey := dvc.rs.pubkey;
-    //         && pred_verify_owner_of_block_share_with_bls_signature(rs_pubkey, block_share)
-    //         ::
-    //         && var dvc: DVCState := dv.honest_nodes_states[hn];
-    //         && inv_block_of_block_shares_is_known_body(dvc, block_share)            
-    // }
+    predicate inv_block_of_block_shares_is_known(
+        dv: DVState
+    )
+    {
+        forall hn: BLSPubkey, block_share: SignedBeaconBlock | 
+            && is_honest_node(dv, hn)
+            && block_share in dv.block_share_network.allMessagesSent 
+            && var dvc: DVCState := dv.honest_nodes_states[hn];
+            && var rs_pubkey: BLSPubkey := dvc.rs.pubkey;
+            && pred_verify_owner_of_block_share_with_bls_signature(rs_pubkey, block_share)
+            ::
+            && var dvc: DVCState := dv.honest_nodes_states[hn];
+            && inv_block_of_block_shares_is_known_body(dvc, block_share)            
+    }
 
-    // predicate inv_proposer_is_created_with_shares_from_quorum_body_signers_helper(
-    //     block_shares: set<BlockShare>,
-    //     dvc: DVCState
-    // )
-    // {
-    //     exists block_share: SignedBeaconBlock ::
-    //         && block_share in block_shares
-    //         && var rs_pubkey := dvc.rs.pubkey;
-    //         && pred_verify_owner_of_block_share_with_bls_signature(rs_pubkey, block_share)
-    // }
+    predicate inv_complete_block_is_created_with_shares_from_quorum_body_signers_helper(
+        block_shares: set<SignedBeaconBlock>,
+        dvc: DVCState
+    )
+    {
+        exists block_share: SignedBeaconBlock ::
+            && block_share in block_shares
+            && var rs_pubkey := dvc.rs.pubkey;
+            && pred_verify_owner_of_block_share_with_bls_signature(rs_pubkey, block_share)
+    }
 
-    // predicate inv_proposer_is_created_with_shares_from_quorum_body_signers(
-    //     dv: DVState,
-    //     block_shares: set<BlockShare>,
-    //     dvc_signer_pubkeys: set<BLSPubkey>
-    // )
-    // {
-    //     forall key: BLSPubkey | key in dvc_signer_pubkeys ::
-    //         key in dv.honest_nodes_states.Keys
-    //         ==>
-    //         inv_proposer_is_created_with_shares_from_quorum_body_signers_helper(
-    //                 block_shares,
-    //                 dv.honest_nodes_states[key]
-    //             )        
-    // }
+    predicate inv_complete_block_is_created_with_shares_from_quorum_body_signers(
+        dv: DVState,
+        block_shares: set<SignedBeaconBlock>,
+        dvc_signer_pubkeys: set<BLSPubkey>
+    )
+    {
+        forall key: BLSPubkey | key in dvc_signer_pubkeys ::
+            key in dv.honest_nodes_states.Keys
+            ==>
+            inv_complete_block_is_created_with_shares_from_quorum_body_signers_helper(
+                    block_shares,
+                    dv.honest_nodes_states[key]
+                )        
+    }
 
-    // predicate inv_proposer_is_created_with_shares_from_quorum_body_helper(
+    // predicate inv_complete_block_is_created_with_shares_from_quorum_body_helper(
     //     dv: DVState, 
-    //     proposer: Block,
-    //     block_shares: set<BlockShare>, 
+    //     block: SignedBeaconBlock,
+    //     block_shares: set<SignedBeaconBlock>, 
     //     signers: set<BLSPubkey>
     // )
     // {
@@ -1811,81 +1896,122 @@ module Block_Inv_With_Empty_Initial_Block_Slashing_DB
     //     && var constructed_sig := dv.construct_complete_signed_block(block_shares);
     //     && constructed_sig.isPresent()
     //     && constructed_sig.safe_get() == proposer.signature
-    //     && all_block_shares_have_the_same_data(block_shares, proposer.data)
+    //     && signed_beacon_blocks_for_the_same_beacon_block(block_shares, block.block)
     //     && signers <= dv.all_nodes
-    //     && inv_proposer_is_created_with_shares_from_quorum_body_signers(dv, block_shares, signers)
+    //     && inv_complete_block_is_created_with_shares_from_quorum_body_signers(dv, block_shares, signers)
     //     && |signers| >= quorum(|dv.all_nodes|)
     // }
 
-    // predicate inv_proposer_is_created_with_shares_from_quorum_body(
-    //     dv: DVState, 
-    //     proposer: Block        
-    // )
-    // {
-    //     exists block_shares, dvc_signer_pubkeys :: 
-    //             && block_shares <= dv.block_share_network.allMessagesSent
-    //             && var constructed_sig := dv.construct_complete_signed_block(block_shares);
-    //             && constructed_sig.isPresent()
-    //             && constructed_sig.safe_get() == proposer.signature
-    //             && all_block_shares_have_the_same_data(block_shares, proposer.data)
-    //             && dvc_signer_pubkeys <= dv.all_nodes
-    //             && inv_proposer_is_created_with_shares_from_quorum_body_signers(dv, block_shares, dvc_signer_pubkeys)
-    //             && |dvc_signer_pubkeys| >= quorum(|dv.all_nodes|)
-    // }
+    predicate inv_complete_block_is_created_with_shares_from_quorum_body_helper(
+        dv: DVState, 
+        complete_block: SignedBeaconBlock,
+        block_shares: set<SignedBeaconBlock>,
+        dvc_signer_pubkeys: set<BLSPubkey>
+    )
+    {
+        && block_shares <= dv.block_share_network.allMessagesSent
+        && dv.construct_complete_signed_block(block_shares).isPresent()
+        && complete_block == dv.construct_complete_signed_block(block_shares).safe_get()
+        && signed_beacon_blocks_for_the_same_beacon_block(block_shares, complete_block.block)
+        && dvc_signer_pubkeys <= dv.all_nodes
+        && inv_complete_block_is_created_with_shares_from_quorum_body_signers(dv, block_shares, dvc_signer_pubkeys)
+        && |dvc_signer_pubkeys| >= quorum(|dv.all_nodes|)
+    }
 
-    // predicate inv_proposer_is_created_with_shares_from_quorum(dv: DVState)
-    // {
-    //     forall proposer: Block | proposer in dv.all_proposers_created ::
-    //             inv_proposer_is_created_with_shares_from_quorum_body(dv, proposer)
-    // }
 
-    // predicate inv_proposer_is_created_with_shares_from_quorum_rs_signers_body(
-    //     block_shares: set<BlockShare>,
-    //     rs_signer_pubkey: BLSPubkey
-    // )
-    // {
-    //     exists block_share: SignedBeaconBlock ::
-    //         && block_share in block_shares
-    //         && pred_verify_owner_of_block_share_with_bls_signature(rs_signer_pubkey, block_share)
-    // }
 
-    // predicate inv_proposer_is_created_with_shares_from_quorum_rs_signers(
-    //     block_shares: set<BlockShare>,
-    //     rs_signer_pubkeys: set<BLSPubkey>
-    // )
-    // {
-    //     forall key: BLSPubkey | key in rs_signer_pubkeys ::
-    //             inv_proposer_is_created_with_shares_from_quorum_rs_signers_body(
-    //                 block_shares,
-    //                 key
-    //             )        
-    // }
+    predicate inv_complete_block_is_created_with_shares_from_quorum_body(
+        dv: DVState, 
+        complete_block: SignedBeaconBlock        
+    )
+    {
+        exists block_shares, dvc_signer_pubkeys ::             
+                && block_shares <= dv.block_share_network.allMessagesSent
+                && dv.construct_complete_signed_block(block_shares).isPresent()
+                && complete_block == dv.construct_complete_signed_block(block_shares).safe_get()
+                && signed_beacon_blocks_for_the_same_beacon_block(block_shares, complete_block.block)
+                && dvc_signer_pubkeys <= dv.all_nodes
+                && inv_complete_block_is_created_with_shares_from_quorum_body_signers(dv, block_shares, dvc_signer_pubkeys)
+                && |dvc_signer_pubkeys| >= quorum(|dv.all_nodes|)
+    }
 
-    // predicate inv_outputs_proposers_submited_is_created_with_shares_from_quorum_body(
-    //     dvc: DVCState, 
-    //     proposer: Block
-    // )
-    // {
-    //     && proposer.data.slot in dvc.rcvd_block_shares.Keys
-    //     && exists block_shares, rs_signer_pubkeys, k ::          
-    //             && k in dvc.rcvd_block_shares[proposer.data.slot].Keys
-    //             && block_shares <= dvc.rcvd_block_shares[proposer.data.slot][k]
-    //             && var constructed_sig := dvc.construct_complete_signed_block(block_shares);
-    //             && constructed_sig.isPresent()
-    //             && constructed_sig.safe_get() == proposer.signature
-    //             && all_block_shares_have_the_same_data(block_shares, proposer.data)
-    //             && inv_proposer_is_created_with_shares_from_quorum_rs_signers(block_shares, rs_signer_pubkeys)
-    //             && |rs_signer_pubkeys| >= quorum(|dvc.peers|)
-    //             && rs_signer_pubkeys <= dvc.peers
-    // }   
+    predicate inv_complete_block_is_created_with_shares_from_quorum(dv: DVState)
+    {
+        forall complete_block: SignedBeaconBlock | complete_block in dv.all_blocks_created ::
+                inv_complete_block_is_created_with_shares_from_quorum_body(dv, complete_block)
+    }
 
-    // predicate inv_outputs_proposers_submited_is_created_with_shares_from_quorum(
-    //     outputs: Outputs,
-    //     dvc: DVCState)
-    // {
-    //     forall submitted_block | submitted_block in outputs.proposers_submitted ::
-    //         inv_outputs_proposers_submited_is_created_with_shares_from_quorum_body(dvc, submitted_block)
-    // } 
+    predicate inv_complete_block_is_created_with_shares_from_quorum_rs_signers_body(
+        block_shares: set<SignedBeaconBlock>,
+        rs_signer_pubkey: BLSPubkey
+    )
+    {
+        exists block_share: SignedBeaconBlock ::
+            && block_share in block_shares
+            && pred_verify_owner_of_block_share_with_bls_signature(rs_signer_pubkey, block_share)
+    }
+
+    predicate inv_complete_block_is_created_with_shares_from_quorum_rs_signers(
+        block_shares: set<SignedBeaconBlock>,
+        rs_signer_pubkeys: set<BLSPubkey>
+    )
+    {
+        forall key: BLSPubkey | key in rs_signer_pubkeys ::
+                inv_complete_block_is_created_with_shares_from_quorum_rs_signers_body(
+                    block_shares,
+                    key
+                )        
+    }
+
+    predicate inv_outputs_blocks_submited_is_created_with_shares_from_quorum_body(
+        dvc: DVCState, 
+        complete_block: SignedBeaconBlock
+    )
+    {
+        && complete_block.block.slot in dvc.rcvd_block_shares.Keys
+        && exists block_shares, rs_signer_pubkeys, k ::          
+                && k in dvc.rcvd_block_shares[complete_block.block.slot].Keys
+                && block_shares <= dvc.rcvd_block_shares[complete_block.block.slot][k]
+                && dvc.construct_complete_signed_block(block_shares).isPresent()
+                && complete_block == dvc.construct_complete_signed_block(block_shares).safe_get()
+                && signed_beacon_blocks_for_the_same_beacon_block(block_shares, complete_block.block)
+                && inv_complete_block_is_created_with_shares_from_quorum_rs_signers(block_shares, rs_signer_pubkeys)
+                && |rs_signer_pubkeys| >= quorum(|dvc.peers|)
+                && rs_signer_pubkeys <= dvc.peers
+    }   
+
+    predicate inv_outputs_blocks_submited_is_created_with_shares_from_quorum(
+        outputs: Outputs,
+        dvc: DVCState)
+    {
+        forall submitted_block | submitted_block in outputs.submitted_blocks ::
+            inv_outputs_blocks_submited_is_created_with_shares_from_quorum_body(dvc, submitted_block)
+    } 
+
+    predicate inv_blocks_of_submitted_signed_block_are_decided_values_body(
+        dv: DVState,
+        complete_block: SignedBeaconBlock
+    )
+    {
+        && complete_block in dv.all_blocks_created
+        && var beacon_block: BeaconBlock := complete_block.block;
+        && var slot := beacon_block.slot;
+        && dv.consensus_instances_on_beacon_block[slot].decided_value.isPresent()
+        && dv.consensus_instances_on_beacon_block[slot].decided_value.safe_get() == beacon_block
+    }
+
+    predicate inv_blocks_of_submitted_signed_block_are_decided_values(
+        dv: DVState
+    )
+    {
+        forall complete_block: SignedBeaconBlock | 
+            complete_block in dv.all_blocks_created
+            ::
+            && var beacon_block: BeaconBlock := complete_block.block;
+            && var slot := beacon_block.slot;
+            && dv.consensus_instances_on_beacon_block[slot].decided_value.isPresent()
+            && dv.consensus_instances_on_beacon_block[slot].decided_value.safe_get() == beacon_block
+    }
 
     // predicate pred_intersection_of_honest_nodes_in_two_quorum_contains_an_honest_node(
     //     dv: DVState,
@@ -1904,110 +2030,197 @@ module Block_Inv_With_Empty_Initial_Block_Slashing_DB
     //         && hn in h_nodes_2
     // }
 
-    // predicate inv_db_of_vp_contains_all_proposer_data_of_sent_block_shares_for_lower_slots_body(
-    //     dv: DVState,
-    //     hn: BLSPubkey,
-    //     slot: Slot, 
-    //     vp: BeaconBlock -> bool, 
-    //     db: set<SlashingDBBlock>
-    // )
-    // {
-    //     forall block_share: SignedBeaconBlock | 
-    //         && block_share in dv.block_share_network.allMessagesSent
-    //         && is_honest_node(dv, hn)
-    //         && var dvc := dv.honest_nodes_states[hn];
-    //         && var rs_pubkey := dvc.rs.pubkey;
-    //         && pred_verify_owner_of_block_share_with_bls_signature(rs_pubkey, block_share)
-    //         && block_share.block.slot < slot
-    //         ::
-    //         && var proposer_data := block_share.block;
-    //         && var slashing_db_proposer := SlashingDBBlock(
-    //                                         source_epoch := proposer_data.source.epoch,
-    //                                         target_epoch := proposer_data.target.epoch,
-    //                                         signing_root := Some(hash_tree_root(proposer_data)));
-    //         && slashing_db_proposer in db
-    // }
+    predicate inv_db_of_vp_contains_all_beacon_block_of_sent_block_shares_for_lower_slots_body(
+        dv: DVState,
+        hn: BLSPubkey,
+        slot: Slot, 
+        vp: BeaconBlock -> bool, 
+        db: set<SlashingDBBlock>
+    )
+    {
+        && is_honest_node(dv, hn) 
+        && var dvc := dv.honest_nodes_states[hn];
+        && var rs_pubkey := dvc.rs.pubkey;
+        && ( forall block_share: SignedBeaconBlock | 
+                && block_share in dv.block_share_network.allMessagesSent
+                && is_honest_node(dv, hn)
+                && pred_verify_owner_of_block_share_with_bls_signature(rs_pubkey, block_share)
+                && block_share.block.slot < slot
+                ::
+                && var beacon_block := block_share.block;
+                && var slashing_db_block := construct_SlashingDBBlock_from_beacon_block(beacon_block);
+                && slashing_db_block in db
+            )
+    }
 
-    // predicate inv_db_of_vp_contains_all_proposer_data_of_sent_block_shares_for_lower_slots(dv: DVState)
-    // {
-    //     forall hn: BLSPubkey, slot: Slot, vp: BeaconBlock -> bool, db: set<SlashingDBBlock> | 
-    //         && is_honest_node(dv, hn) 
-    //         && var dvc := dv.honest_nodes_states[hn];
-    //         && slot in dvc.block_consensus_engine_state.block_slashing_db_hist
-    //         && vp in dvc.block_consensus_engine_state.block_slashing_db_hist[slot]
-    //         && db in dvc.block_consensus_engine_state.block_slashing_db_hist[slot][vp]
-    //         :: 
-    //         inv_db_of_vp_contains_all_proposer_data_of_sent_block_shares_for_lower_slots_body(
-    //             dv,
-    //             hn,
-    //             slot,
-    //             vp,
-    //             db)
-    // }
+    predicate inv_db_of_vp_contains_all_beacon_block_of_sent_block_shares_for_lower_slots_helper(
+        dv: DVState,
+        hn: BLSPubkey
+    )
+    {
+        && is_honest_node(dv, hn) 
+        && var dvc := dv.honest_nodes_states[hn];
+        && forall slot: Slot, vp: BeaconBlock -> bool, db: set<SlashingDBBlock> | 
+                && slot in dvc.block_consensus_engine_state.block_slashing_db_hist
+                && vp in dvc.block_consensus_engine_state.block_slashing_db_hist[slot]
+                && db in dvc.block_consensus_engine_state.block_slashing_db_hist[slot][vp]
+                :: 
+                inv_db_of_vp_contains_all_beacon_block_of_sent_block_shares_for_lower_slots_body(
+                    dv,
+                    hn,
+                    slot,
+                    vp,
+                    db)
+    }
 
-    // predicate inv_db_of_vp_contains_all_proposer_data_of_sent_block_shares_for_lower_slots_body_dvc(
-    //     allMessagesSent: set<BlockShare>,
-    //     rs_pubkey: BLSPubkey,
-    //     slot: Slot, 
-    //     vp: BeaconBlock -> bool, 
-    //     db: set<SlashingDBBlock>
-    // )
-    // {
-    //     forall block_share: SignedBeaconBlock | 
-    //         && block_share in allMessagesSent
-    //         && pred_verify_owner_of_block_share_with_bls_signature(rs_pubkey, block_share)
-    //         && block_share.block.slot < slot
-    //         ::
-    //         && var proposer_data := block_share.block;
-    //         && var slashing_db_proposer := SlashingDBBlock(
-    //                                         source_epoch := proposer_data.source.epoch,
-    //                                         target_epoch := proposer_data.target.epoch,
-    //                                         signing_root := Some(hash_tree_root(proposer_data)));
-    //         && slashing_db_proposer in db
-    // }
+    predicate inv_db_of_vp_contains_all_beacon_block_of_sent_block_shares_for_lower_slots(dv: DVState)
+    {
+        forall hn: BLSPubkey | is_honest_node(dv, hn) 
+            ::
+            inv_db_of_vp_contains_all_beacon_block_of_sent_block_shares_for_lower_slots_helper(dv, hn)
+    }
 
-    // predicate inv_db_of_vp_contains_all_proposer_data_of_sent_block_shares_for_lower_slots_dvc(
-    //     allMessagesSent: set<BlockShare>,
-    //     dvc: DVCState        
-    // )
-    // {
-    //     forall slot: Slot, vp: BeaconBlock -> bool, db: set<SlashingDBBlock> | 
-    //         && slot in dvc.block_consensus_engine_state.block_slashing_db_hist
-    //         && vp in dvc.block_consensus_engine_state.block_slashing_db_hist[slot]
-    //         && db in dvc.block_consensus_engine_state.block_slashing_db_hist[slot][vp]
-    //         :: 
-    //         inv_db_of_vp_contains_all_proposer_data_of_sent_block_shares_for_lower_slots_body_dvc(
-    //             allMessagesSent,
-    //             dvc.rs.pubkey,
-    //             slot,
-    //             vp,
-    //             db
-    //         )
-    // }
+    predicate inv_db_of_vp_from_block_share_contains_all_beacon_block_of_sent_block_shares_for_lower_slots_dvc_body_conclusion(
+        allMessagesSent: set<SignedBeaconBlock>,
+        rs_pubkey: BLSPubkey,
+        slot: Slot, 
+        vp: BeaconBlock -> bool, 
+        db: set<SlashingDBBlock>,
+        block_share: SignedBeaconBlock
+    )
+    {
+        && var beacon_block := block_share.block;
+        && var slashing_db_block := construct_SlashingDBBlock_from_beacon_block(beacon_block);        
+        && slashing_db_block in db
+    }
 
-    // predicate inv_unchanged_dvc_rs_pubkey(dv: DVState)
-    // {
-    //     forall hn: BLSPubkey | is_honest_node(dv, hn) ::
-    //         && var dvc: DVCState := dv.honest_nodes_states[hn];
-    //         && dvc.rs.pubkey == hn
-    // }
+    predicate inv_db_of_vp_from_block_share_contains_all_beacon_block_of_sent_block_shares_for_lower_slots_dvc_body(
+        allMessagesSent: set<SignedBeaconBlock>,
+        rs_pubkey: BLSPubkey,
+        slot: Slot, 
+        vp: BeaconBlock -> bool, 
+        db: set<SlashingDBBlock>
+    )
+    {
+        forall block_share: SignedBeaconBlock | 
+            && block_share in allMessagesSent
+            && pred_verify_owner_of_block_share_with_bls_signature(rs_pubkey, block_share)
+            && block_share.block.slot < slot
+            ::
+            inv_db_of_vp_from_block_share_contains_all_beacon_block_of_sent_block_shares_for_lower_slots_dvc_body_conclusion(
+                allMessagesSent,
+                rs_pubkey,
+                slot,
+                vp,
+                db,
+                block_share
+            )
+    }
 
-    // predicate inv_honest_nodes_are_not_owner_of_block_shares_from_adversary_body(
-    //     dv: DVState, 
-    //     block_share: SignedBeaconBlock
-    // )
-    // {
-    //     forall hn: BLSPubkey | is_honest_node(dv, hn) :: 
-    //         !pred_verify_owner_of_block_share_with_bls_signature(hn, block_share)
-    // }
+    predicate inv_db_of_vp_from_block_share_contains_all_beacon_block_of_sent_block_shares_for_lower_slots_dvc(
+        allMessagesSent: set<SignedBeaconBlock>,
+        dvc: DVCState        
+    )
+    {
+        forall slot: Slot, vp: BeaconBlock -> bool, db: set<SlashingDBBlock> | 
+            && slot in dvc.block_consensus_engine_state.block_slashing_db_hist
+            && vp in dvc.block_consensus_engine_state.block_slashing_db_hist[slot]
+            && db in dvc.block_consensus_engine_state.block_slashing_db_hist[slot][vp]
+            :: 
+            inv_db_of_vp_from_block_share_contains_all_beacon_block_of_sent_block_shares_for_lower_slots_dvc_body(
+                allMessagesSent,
+                dvc.rs.pubkey,
+                slot,
+                vp,
+                db
+            )
+    }
 
-    // predicate inv_honest_nodes_are_not_owner_of_block_shares_from_adversary(dv: DVState)
-    // {
-    //     forall byz_node: BLSPubkey, block_share: SignedBeaconBlock | 
-    //         && byz_node in dv.adversary.nodes 
-    //         && block_share in dv.block_share_network.allMessagesSent
-    //         && pred_verify_owner_of_block_share_with_bls_signature(byz_node, block_share)
-    //         ::
-    //         inv_honest_nodes_are_not_owner_of_block_shares_from_adversary_body(dv, block_share)
-    // }
+    predicate inv_unchanged_dvc_rs_pubkey(dv: DVState)
+    {
+        forall hn: BLSPubkey | is_honest_node(dv, hn) ::
+            && var dvc: DVCState := dv.honest_nodes_states[hn];
+            && dvc.rs.pubkey == hn
+    }
+
+    predicate inv_honest_nodes_are_not_owner_of_block_shares_from_adversary_body(
+        dv: DVState, 
+        block_share: SignedBeaconBlock
+    )
+    {
+        forall hn: BLSPubkey | is_honest_node(dv, hn) :: 
+            !pred_verify_owner_of_block_share_with_bls_signature(hn, block_share)
+    }
+
+    predicate inv_honest_nodes_are_not_owner_of_block_shares_from_adversary(dv: DVState)
+    {
+        forall byz_node: BLSPubkey, block_share: SignedBeaconBlock | 
+            && byz_node in dv.adversary.nodes 
+            && block_share in dv.block_share_network.allMessagesSent
+            && pred_verify_owner_of_block_share_with_bls_signature(byz_node, block_share)
+            ::
+            inv_honest_nodes_are_not_owner_of_block_shares_from_adversary_body(dv, block_share)
+    }
+
+    predicate inv_stored_SlashingDBBlocks_have_available_signing_root_body(dvc: DVCState)
+    {
+        forall slashing_db_block: SlashingDBBlock | 
+                slashing_db_block in dvc.block_slashing_db
+                ::
+                slashing_db_block.signing_root.isPresent()
+    }
+
+    predicate inv_stored_SlashingDBBlocks_have_available_signing_root(dv: DVState)
+    {
+        forall hn | is_honest_node(dv, hn) ::
+            inv_stored_SlashingDBBlocks_have_available_signing_root_body(dv.honest_nodes_states[hn])
+    }
+
+    
+
+    predicate inv_at_most_submitted_signed_beacon_block_for_every_slot(dv: DVState)
+    {
+        forall sbb1, sbb2: SignedBeaconBlock |
+            && sbb1 in dv.all_blocks_created
+            && sbb2 in dv.all_blocks_created
+            && sbb1.block.slot == sbb2.block.slot
+            ::
+            && var bb1 := sbb1.block;
+            && var bb2 := sbb2.block;
+            && var sdbb1 := construct_SlashingDBBlock_from_beacon_block(bb1);
+            && var sdbb2 := construct_SlashingDBBlock_from_beacon_block(bb2);
+            && sdbb1.signing_root.isPresent()
+            && sdbb2.signing_root.isPresent()
+            && sdbb1.signing_root.safe_get() == sdbb2.signing_root.safe_get()
+    }
+
+    predicate inv_slots_in_slashing_db_is_not_higher_than_slot_of_latest_proposer_duty_body(dvc: DVCState)
+    {   
+        dvc.latest_proposer_duty.isPresent()
+        ==>
+        ( && var slot := dvc.latest_proposer_duty.safe_get().slot;
+          && forall slashing_db_block: SlashingDBBlock | slashing_db_block in dvc.block_slashing_db
+                ::
+                slashing_db_block.slot <= slot
+        )
+    }
+
+    predicate inv_slots_in_slashing_db_is_not_higher_than_slot_of_latest_proposer_duty(dv: DVState)
+    {
+        forall hn | is_honest_node(dv, hn) ::
+            inv_slots_in_slashing_db_is_not_higher_than_slot_of_latest_proposer_duty_body(dv.honest_nodes_states[hn])
+    }
+
+    predicate inv_none_latest_proposer_duty_implies_emply_block_slashing_db_body(dvc: DVCState)
+    {
+        !dvc.latest_proposer_duty.isPresent()
+        ==>
+        dvc.block_slashing_db == {}
+    }
+
+    predicate inv_none_latest_proposer_duty_implies_emply_block_slashing_db(dv: DVState)
+    {
+        forall hn | is_honest_node(dv, hn) ::
+            inv_none_latest_proposer_duty_implies_emply_block_slashing_db_body(dv.honest_nodes_states[hn])
+    }
 }
